@prefix : <http://www.semanticweb.org/cco/> .
@prefix cco: <https://www.commoncoreontologies.org/> .
@prefix BFO: <http://purl.obolibrary.org/obo/> .
@prefix owl: <http://www.w3.org/2002/07/owl#> .
@prefix rdf: <http://www.w3.org/1999/02/22-rdf-syntax-ns#> .
@prefix rdfs: <http://www.w3.org/2000/01/rdf-schema#> .
@prefix xsd: <http://www.w3.org/2001/XMLSchema#> .

<http://www.semanticweb.org/cco/> rdf:type owl:Ontology .

#################################################################
#    Object Properties
#################################################################

# bearer_of (RO_0000053)
:bearer_of rdf:type owl:ObjectProperty ;
    rdfs:label "bearer of"@en .

# realized_by (BFO_0000054)
BFO:BFO_0000054 rdf:type owl:ObjectProperty ;
    rdfs:label "realized by"@en .

# has_participant (BFO_0000057)
BFO:BFO_0000057 rdf:type owl:ObjectProperty ;
    rdfs:label "has participant"@en .

#################################################################
#    Classes
#################################################################

# BFO Process
BFO:BFO_0000015 rdf:type owl:Class ;
    rdfs:label "process"@en .

# Artifacts

cco:ont00001242 rdf:type owl:Class ;
  rdfs:subClassOf :Transducer ;
  rdfs:label "Actuator"@en ;
  rdfs:comment "Actuator is a Transducer that is designed to convert some control signal into mechanical motion."@en .

cco:ont00000524 rdf:type owl:Class ;
  rdfs:subClassOf :CoolingSystem ;
  rdfs:label "Air Conditioning Unit"@en ;
  rdfs:comment "Air Conditioning Unit is a Cooling System that is designed to remove excess heat and humidity from the air in an enclosed space."@en .

cco:ont00000111 rdf:type owl:Class ;
  rdfs:subClassOf :FluidControlArtifact ;
  rdfs:label "Air Inlet"@en ;
  rdfs:comment "Air Inlet is a Fluid Control Artifact that consists of an opening that is designed to capture and direct the flow of air into the system it is part of."@en .

cco:ont00001083 rdf:type owl:Class ;
  rdfs:subClassOf :ReactionEngine ;
  rdfs:label "Air-Breathing Combustion Engine"@en ;
  rdfs:comment "Air-Breathing Combustion Engine is a Reaction Engine that functions by drawing a continuous stream of air into and through the Engine where it is compressed, mixed with a Portion of Fuel, ignited, and then expelled as exhaust gas."@en .

cco:ont00000294 rdf:type owl:Class ;
  rdfs:subClassOf :JetEngine ;
  rdfs:label "Air-Breathing Jet Engine"@en ;
  rdfs:comment "Air-Breathing Jet Engine is a Jet Engine that is propelled by a jet of hot exhaust gases formed from air that is drawn into the Engine via an Air Inlet."@en .

cco:ont00001043 rdf:type owl:Class ;
  rdfs:subClassOf :Vehicle ;
  rdfs:label "Aircraft"@en ;
  rdfs:comment "Aircraft is a Vehicle that is designed to convey passengers, cargo, or equipment from one location to another by air travel."@en .

cco:ont00001229 rdf:type owl:Class ;
  rdfs:subClassOf :PrimaryCellElectricBattery ;
  rdfs:label "Alkaline Electric Battery"@en ;
  rdfs:comment "Alkaline Electric Battery is a Primary Cell Electric Battery that has a Zinc anode and Manganese (IV) oxide cathode."@en .

cco:ont00000302 rdf:type owl:Class ;
  rdfs:subClassOf :ElectricalPowerSource ,
        [ rdf:type owl:Restriction ;
      owl:onProperty :bearer_of ;
      owl:someValuesFrom cco:ont00000994
    ] ;
  rdfs:label "Alternating Current Power Source"@en ;
  rdfs:comment "Alternating Current Power Source is an Electrical Power Source that is designed to transfer electrical power in the form of alternating current."@en .

cco:ont00000427 rdf:type owl:Class ;
  rdfs:subClassOf :GroundMotorVehicle ;
  rdfs:label "Armored Fighting Vehicle"@en ;
  rdfs:comment "Armored Fighting Vehicle is a Ground Motor Vehicle that is designed to be armored and used to transport and support military personal in combat missions."@en .

cco:ont00000467 rdf:type owl:Class ;
  rdfs:subClassOf :ArmoredFightingVehicle ;
  rdfs:label "Armored Personnel Carrier"@en ;
  rdfs:comment "Armored Personnel Carrier is an Armored Fighting Vehicle that is designed to transport infantry to the battlefield but which are not usually designed to take part in a direct-fire battle."@en .

cco:ont00000178 rdf:type owl:Class ;
  rdfs:subClassOf :PortionofAmmunition ;
  rdfs:label "Arrow"@en ;
  rdfs:comment "Arrow is a Portion of Ammunition that is designed to be fired from a Bow and consists of a long straight stiff shaft with stabilizers (fletchings) and a slot (the nock) on one end and a weighted tip (the arrowhead) on the other end."@en .

cco:ont00001313 rdf:type owl:Class ;
  rdfs:subClassOf :MaterialArtifact ;
  rdfs:label "Article of Clothing"@en ;
  rdfs:comment "Article of Clothing is a Material Artifact that is designed to cover some portion of a body."@en .

cco:ont00000571 rdf:type owl:Class ;
  rdfs:subClassOf :PortionofWasteMaterial ;
  rdfs:label "Article of Solid Waste"@en ;
  rdfs:comment "Article of Solid Waste is a Portion of Waste Material that has a low liquid content."@en .

cco:ont00000319 rdf:type owl:Class ;
  rdfs:subClassOf :DirectiveInformationContentEntity ;
  rdfs:label "Artifact Design"@en ;
  rdfs:comment "Artifact Design is a Directive Information Content Entity that is a specification of an object, manifested by an agent, intended to accomplish goals, in a particular environment, using a set of primitive components, satisfying a set of requirements, subject to constraints."@en .

cco:ont00000856 rdf:type owl:Class ;
  rdfs:label "Artifact History"@en ;
  rdfs:comment "Artifact History is a History of an Artifact."@en .

cco:ont00000292 rdf:type owl:Class ;
  rdfs:subClassOf :DesignativeInformationContentEntity ;
  rdfs:label "Artifact Identifier"@en ;
  rdfs:comment "Artifact Identifier is a Designative Information Content Entity that designates some Artifact."@en .

cco:ont00000591 rdf:type owl:Class ;
  rdfs:subClassOf :Site ;
  rdfs:label "Artifact Location"@en ;
  rdfs:comment "Artifact Location is a Site that is the location of some Artifact."@en .

cco:ont00001045 rdf:type owl:Class ;
  rdfs:subClassOf :DirectiveInformationContentEntity ;
  rdfs:label "Artifact Model"@en ;
  rdfs:comment "Artifact Model is a Directive Information Content Entity that prescribes a common set of Functions and Qualities to inhere in a set of artifact instances."@en .

cco:ont00001103 rdf:type owl:Class ;
  rdfs:subClassOf :DesignativeInformationContentEntity ;
  rdfs:label "Artifact Model Name"@en ;
  rdfs:comment "Artifact Model Name is a Designative Information Content Entity that designates some Artifact Model."@en .

cco:ArtifactOntology rdf:type owl:Class ;
  rdfs:label "Artifact Ontology"@en ;
  rdfs:comment "Artifact Ontology is described as: nan."@en .

cco:ont00001248 rdf:type owl:Class ;
  rdfs:subClassOf :Prosthesis ;
  rdfs:label "Artificial Eye"@en ;
  rdfs:comment "Artificial Eye is a Prosthesis that is designed to replace a missing eye."@en .

cco:ont00000968 rdf:type owl:Class ;
  rdfs:subClassOf :Rifle ;
  rdfs:label "Assault Rifle"@en ;
  rdfs:comment "Assault Rifle is a Rifle that is designed to have selective-fire functionality and use an intermediate Cartridge and a detachable magazine."@en .

cco:ont00001011 rdf:type owl:Class ;
  rdfs:label "Automobile"@en ;
  rdfs:comment "A Ground Motor Vehicle that is designed to transport a small number of passengers on roads."@en .

cco:ont00000086 rdf:type owl:Class ;
  rdfs:subClassOf :VehicleControlSystem ;
  rdfs:label "Autopilot System"@en ;
  rdfs:comment "Autopilot System is a Vehicle Control System that is designed to enable some Agent to control the trajectory of a Vehicle without constant 'hands-on' control."@en .

cco:ont00000049 rdf:type owl:Class ;
  rdfs:label "Banknote"@en ;
  rdfs:comment "A Portion of Cash that consists of a portable slip of paper or fabric designed to bear some specified Financial Value."@en .

cco:ont00000668 rdf:type owl:Class ;
  rdfs:subClassOf :MaterialArtifact ;
  rdfs:label "Battery Terminal"@en ;
  rdfs:comment "Battery Terminal is a Material Artifact that is designed to connect a load or charger to a single or multiple-cell Battery."@en .

cco:ont00001138 rdf:type owl:Class ;
  rdfs:subClassOf :WireAntenna ;
  rdfs:label "Beverage Antenna"@en ;
  rdfs:comment "Beverage Antenna is a Wire Antenna that consists of a horizontal wire one-half to two wavelengths long that is suspended above the ground with one end attached to the receiver feedline and the other grounded and which is typically used in the low and medium frequency radio bands."@en .

cco:ont00000840 rdf:type owl:Class ;
  rdfs:subClassOf :GroundVehicle ,
        [ rdf:type owl:Restriction ;
      owl:onProperty :bearer_of ;
      owl:someValuesFrom cco:ont00000994
    ] ;
  rdfs:label "Bicycle"@en ;
  rdfs:comment "Bicycle is a Ground Vehicle that consists of two wheels, one in front of the other, attached to a frame along with handlebars and pedals such that it is designed to receive its motive power from pedaling."@en .

cco:ont00000092 rdf:type owl:Class ;
  rdfs:subClassOf :Transducer ;
  rdfs:label "Bidirectional Transducer"@en ;
  rdfs:comment "Bidirectional Transducer is a Transducer that is designed to receive a signal in the form of physical phenomena and convert it into an electrical signal, and vice versa."@en .

cco:ont00001008 rdf:type owl:Class ;
  rdfs:subClassOf :Weapon ;
  rdfs:label "Biological Weapon"@en ;
  rdfs:comment "Biological Weapon is a Weapon that is designed to inflict harm, incapacity, or death by means of releasing disease-producing agentsâ€”such as bacteria, viruses, or fungi."@en .

cco:ont00001159 rdf:type owl:Class ;
  rdfs:subClassOf :FinancialInstrument ;
  rdfs:label "Bond"@en ;
  rdfs:comment "Bond is a Financial Instrument that is designed to secure an Agent's debt for the holders of that debt."@en .

cco:ont00000536 rdf:type owl:Class ;
  rdfs:subClassOf :Bond ;
  rdfs:label "Bond Certificate"@en ;
  rdfs:comment "Bond Certificate is a Bond that consists of a Certificate."@en .

cco:ont00001373 rdf:type owl:Class ;
  rdfs:subClassOf :ProjectileLauncher ;
  rdfs:label "Bow"@en ;
  rdfs:comment "Bow is a Projectile Launcher that is designed to launch Arrows."@en .

cco:ont00000342 rdf:type owl:Class ;
  rdfs:subClassOf     [ rdf:type owl:Restriction ;
      owl:onProperty :bearer_of ;
      owl:someValuesFrom cco:ont00001155
    ] ;
  rdfs:label "Brake"@en ;
  rdfs:comment "A Material Artifact that is designed to inhibit motion in a moving system by absorbing or dissipating energy (e.g., in vehicles or machinery)."@en .

cco:ont00000877 rdf:type owl:Class ;
  rdfs:subClassOf :VehicleControlSystem ,
        [ rdf:type owl:Restriction ;
      owl:onProperty :bearer_of ;
      owl:someValuesFrom cco:ont00000679
    ] ;
  rdfs:label "Brake Control System"@en ;
  rdfs:comment "Brake Control System is a Vehicle Control System that is designed to control the process of braking with the aim of preventing rolling, skidding, and hydroplaning."@en .

cco:ont00001099 rdf:type owl:Class ;
  rdfs:label "Bridge"@en ;
  rdfs:comment "A Land Transportation Artifact that is designed to span physical obstacles such as land or water while maintaining passage beneath, enabling persons and vehicles to pass over the obstacle."@en .

cco:ont00000748 rdf:type owl:Class ;
  rdfs:subClassOf :PortionofAmmunition ;
  rdfs:label "Bullet"@en ;
  rdfs:comment "Bullet is a Portion of Ammunition that is designed to be projected by a Firearm, Sling, Slingshot, or Air Gun, but which does not (typically) contain explosives."@en .

cco:ont00001292 rdf:type owl:Class ;
  rdfs:label "Bus"@en ;
  rdfs:comment "A Ground Motor Vehicle that is designed to transport many passengers on roads; wheel and axle configurations may vary."@en .

cco:ont00001249 rdf:type owl:Class ;
  rdfs:subClassOf :EnvironmentControlSystem ,
        [ rdf:type owl:Restriction ;
      owl:onProperty :bearer_of ;
      owl:someValuesFrom cco:ont00000679
    ] ;
  rdfs:label "Cabin Pressurization Control System"@en ;
  rdfs:comment "Cabin Pressurization Control System is an Environment Control System that is designed to control the process in which conditioned air is pumped into the Cabin of some Aircraft or Spacecraft in order to create a safe and comfortable environment for passengers and crew flying at high altitudes."@en .

cco:ont00000199 rdf:type owl:Class ;
  rdfs:subClassOf :ImagingInstrument ;
  rdfs:label "Camera"@en ;
  rdfs:comment "Camera is an Imaging Instrument that is designed to form and digitally or physically record an image of an entity."@en .

cco:ont00000747 rdf:type owl:Class ;
  rdfs:subClassOf :WaterTransportationArtifact ;
  rdfs:label "Canal"@en ;
  rdfs:comment "Canal is a Water Transportation Artifact that is an artificial Hydrographic Feature designed to convey water or enable Watercraft to travel inland."@en .

cco:ont00000268 rdf:type owl:Class ;
  rdfs:subClassOf :ProjectileLauncher ;
  rdfs:label "Cannon"@en ;
  rdfs:comment "Cannon is a Projectile Launcher that is designed to use a controlled explosion to launch a relatively large Portion of Ammunition, such as a Round Shot or a Shell, at a significant Velocity."@en .

cco:ont00000143 rdf:type owl:Class ;
  rdfs:subClassOf :VehicleCompartment ;
  rdfs:label "Cargo Cabin"@en ;
  rdfs:comment "Cargo Cabin is a Vehicle Compartment that is used to store goods or materials during transportation."@en .

cco:ont00001003 rdf:type owl:Class ;
  rdfs:subClassOf :PortionofAmmunition ;
  rdfs:label "Cartridge"@en ;
  rdfs:comment "Cartridge is a Portion of Ammunition that is designed to package a Bullet, a propellant substance, and a primer within a case that is designed to fit within the firing chamber of a Firearm."@en .

cco:ont00000792 rdf:type owl:Class ;
  rdfs:subClassOf :OpticalTelescope ;
  rdfs:label "Catadioptric Optical Telescope"@en ;
  rdfs:comment "Catadioptric Optical Telescope is an Optical Telescope that is designed to aid in the observation of spatially distant Objects by means of collecting and focusing visible light through the use of a combination of Lenses and Mirrors to form an enhanced image of the Object."@en .

cco:ont00001095 rdf:type owl:Class ;
  rdfs:label "Cellular Telecommunication Network"@en ;
  rdfs:comment "Cellular Telecommunication Network is a Wireless Telecommunication Network where the last link between the network and the end user is wireless and is distributed over service areas called cells."@en .

cco:ont00000212 rdf:type owl:Class ;
  rdfs:subClassOf :Weapon ;
  rdfs:label "Chemical Weapon"@en ;
  rdfs:comment "Chemical Weapon is a Weapon that is designed to inflict harm, damage, or incapacity by means of releasing toxic chemicals."@en .

cco:ont00001343 rdf:type owl:Class ;
  rdfs:subClassOf :MaterialArtifact ;
  rdfs:label "Circuit Breaker"@en ;
  rdfs:comment "Circuit Breaker is a Material Artifact that is designed to protect an electrical circuit from damage caused by excess current from an overload or short circuit."@en .

cco:ont00001093 rdf:type owl:Class ;
  rdfs:label "Coin"@en ;
  rdfs:comment "A Portion of Cash that consists of a flat, portable, round piece of metal designed to bear some specified Financial Value."@en .

cco:ont00000397 rdf:type owl:Class ;
  rdfs:subClassOf :MaterialArtifact ;
  rdfs:label "Combustion Chamber"@en ;
  rdfs:comment "Combustion Chamber is a Material Artifact that is designed to wholly or partially bound an internal Site where a Combustion process is intended to occur."@en .

cco:ont00000746 rdf:type owl:Class ;
  rdfs:subClassOf :HeatEngine ;
  rdfs:label "Combustion Engine"@en ;
  rdfs:comment "Combustion Engine is a Heat Engine that is designed to convert thermal energy that is generated through a local Combustion process into mechanical energy."@en .

cco:ont00001097 rdf:type owl:Class ;
  rdfs:subClassOf :Stock ;
  rdfs:label "Common Stock"@en ;
  rdfs:comment "Common Stock is a Stock that entitles its holder to voting on corporate decisions."@en .

cco:ont00000346 rdf:type owl:Class ;
  rdfs:subClassOf :MaterialArtifact ,
        [ rdf:type owl:Restriction ;
      owl:onProperty :bearer_of ;
      owl:someValuesFrom cco:ont00000727
    ] ;
  rdfs:label "Communication Instrument"@en ;
  rdfs:comment "Communication Instrument is a Material Artifact that is designed to facilitate communication between at least two entities."@en .

cco:ont00001036 rdf:type owl:Class ;
  rdfs:subClassOf :MaterialArtifact ;
  rdfs:label "Communication System"@en ;
  rdfs:comment "Communication System is a Material Artifact that is designed to enable some Act of Communication by means of transmission systems, relay stations, tributary stations, and data terminal equipment, usually capable of interconnection and interoperation to form an integrated whole."@en .

cco:ont00000097 rdf:type owl:Class ;
  rdfs:label "Complex Optical Lens"@en ;
  rdfs:comment "An Optical Lens consisting of more than one Simple Optical Lens."@en .

cco:ont00000758 rdf:type owl:Class ;
  rdfs:subClassOf :Role ;
  rdfs:label "Component Role"@en ;
  rdfs:comment "Component Role is a Role that inheres in an entity having a discrete structure in virtue of that entity being part of a system considered at a particular level of analysis."@en .

cco:ont00000807 rdf:type owl:Class ;
  rdfs:subClassOf :InternalCombustionEngine ;
  rdfs:label "Compression Ignition Engine"@en ;
  rdfs:comment "Compression Ignition Engine is an Internal Combustion Engine that is designed to operate by igniting a portion of Fuel and Oxidizer mixture using heat generated via compression of the mixture."@en .

cco:ont00000454 rdf:type owl:Class ;
  rdfs:subClassOf :IgnitionSystem ;
  rdfs:label "Compression Ignition System"@en ;
  rdfs:comment "Compression Ignition System is an Ignition System that is designed to generate heat by compressing a portion of fuel and oxidizer mixture in order to initiate an Ignition process."@en .

cco:ont00000420 rdf:type owl:Class ;
  rdfs:subClassOf :InformationProcessingArtifact ;
  rdfs:label "Computer"@en ;
  rdfs:comment "Computer is an Information Processing Artifact that is designed to execute an arbitrary set of arithmetic or logical operations automatically."@en .

cco:ont00000700 rdf:type owl:Class ;
  rdfs:subClassOf :TelecommunicationNetwork ;
  rdfs:label "Computer Network"@en ;
  rdfs:comment "Computer Network is a Telecommunication Network that is designed to allow the exchange of data between two or more computers connected to the network."@en .

cco:ont00000020 rdf:type owl:Class ;
  rdfs:subClassOf :MaterialArtifact ;
  rdfs:label "Container"@en ;
  rdfs:comment "Container is a Material Artifact that is designed to contain (wholly or partially) some material entity."@en .

cco:ont00000095 rdf:type owl:Class ;
  rdfs:subClassOf :MaterialArtifact ;
  rdfs:label "Control Surface"@en ;
  rdfs:comment "Control Surface is a Material Artifact that is designed to deflect air, water, or another medium around its surface in order to change the Attitude of a Vehicle by rotating the Vehicle on one or more of its Axes of Rotation."@en .

cco:ont00000781 rdf:type owl:Class ;
  rdfs:subClassOf :MaterialArtifact ;
  rdfs:label "Control System"@en ;
  rdfs:comment "Control System is a Material Artifact that is designed to manage, command, direct, or regulate the behavior of at least one other Artifact."@en .

cco:ont00000586 rdf:type owl:Class ;
  rdfs:subClassOf :Propellerwhosebladesare ;
  rdfs:label "Controllable Pitch Propeller"@en ;
  rdfs:comment "Controllable Pitch Propeller is a Propeller whose blades are designed to be alterable by rotating the blades about their vertical axis by means of mechanical or hydraulic arrangement."@en .

cco:ont00001015 rdf:type owl:Class ;
  rdfs:subClassOf :Highway ;
  rdfs:label "Controlled-Access Highway"@en ;
  rdfs:comment "Controlled-Access Highway is a Highway that is designed for high-speed vehicular traffic, with all traffic flow and ingress/egress regulated."@en .

cco:ont00000698 rdf:type owl:Class ;
  rdfs:subClassOf :Nozzle ;
  rdfs:label "Convergent-Divergent Nozzle"@en ;
  rdfs:comment "Convergent-Divergent Nozzle is a Nozzle that consists of a tube with an asymmetric hourglass shape that is designed to accelerate hot pressurized gas by converting the heat energy of the gas flow into kinetic energy as it passes through the Nozzle Throat to generate increased Exhaust Velocity of the gas as it exits the Nozzle."@en .

cco:ont00000350 rdf:type owl:Class ;
  rdfs:subClassOf :EnvironmentControlSystem ;
  rdfs:label "Cooling System"@en ;
  rdfs:comment "Cooling System is an Environment Control System that is designed to cool the air or objects in a Site."@en .

cco:ont00000282 rdf:type owl:Class ;
  rdfs:subClassOf :CounterfeitInstrument ;
  rdfs:label "Counterfeit Financial Instrument"@en ;
  rdfs:comment "Counterfeit Financial Instrument is a Counterfeit Instrument that is designed to be a fake replica of some legally sanctioned Financial Instrument."@en .

cco:ont00000719 rdf:type owl:Class ;
  rdfs:subClassOf :MaterialArtifact ;
  rdfs:label "Counterfeit Instrument"@en ;
  rdfs:comment "Counterfeit Instrument is a Material Artifact that is designed to be a fake replica of some genuine Artifact."@en .

cco:ont00001161 rdf:type owl:Class ;
  rdfs:subClassOf :CounterfeitInstrument ;
  rdfs:label "Counterfeit Legal Instrument"@en ;
  rdfs:comment "Counterfeit Legal Instrument is a Counterfeit Instrument that is designed to be a fake replica of some genuine Legal Instrument."@en .

cco:ont00000458 rdf:type owl:Class ;
  rdfs:subClassOf :MaterialArtifact ;
  rdfs:label "Coupling"@en ;
  rdfs:comment "Coupling is a Material Artifact that is designed to connect two Shafts together at their ends for the purpose of transmitting power."@en .

cco:ont00000720 rdf:type owl:Class ;
  rdfs:subClassOf :Container ;
  rdfs:label "Cryogenic Storage Dewar"@en ;
  rdfs:comment "Cryogenic Storage Dewar is a Container that is designed to store a Portion of Cryogenic Material (such as liquid helium or liquid oxygen) and which consists of, minimally, walls that are constructed from two or more layers that are separated by a high vacuum to provide thermal insulation between the interior and exterior of the dewar."@en .

cco:ont00000081 rdf:type owl:Class ;
  rdfs:subClassOf :Weapon ;
  rdfs:label "Cutting Weapon"@en ;
  rdfs:comment "Cutting Weapon is a Weapon that is designed to inflict harm, damage, or incapacity by means of separating some portion of its target into two or more portions through the application of acutely directed force."@en .

cco:ont00000561 rdf:type owl:Class ;
  rdfs:subClassOf :MaterialArtifact ;
  rdfs:label "Dam"@en ;
  rdfs:comment "Dam is a Material Artifact that is designed to impound surface water or underground streams."@en .

cco:ont00000652 rdf:type owl:Class ;
  rdfs:subClassOf :MaterialArtifact ;
  rdfs:label "Decoy"@en ;
  rdfs:comment "Decoy is a Material Artifact that is designed to distract or conceal what an individual or group might be looking for."@en .

cco:ont00000001 rdf:type owl:Class ;
  rdfs:subClassOf :Prism ;
  rdfs:label "Deflecting Prism"@en ;
  rdfs:comment "Deflecting Prism is a Prism designed to deflect a beam of light entering the Prism by a fixed angle."@en .

cco:ont00001188 rdf:type owl:Class ;
  rdfs:subClassOf :Prosthesis ;
  rdfs:label "Denture"@en ;
  rdfs:comment "Denture is a Prosthesis that is designed to replace missing teeth."@en .

cco:ont00000686 rdf:type owl:Class ;
  rdfs:subClassOf :InformationContentEntity ;
  rdfs:label "Designative Information Content Entity"@en ;
  rdfs:comment "Designative Information Content Entity is an Information Content Entity that consists of a set of symbols that denote some Entity."@en .

cco:ont00000230 rdf:type owl:Class ;
  rdfs:subClassOf :OpticalInstrumentwithaperiodicstructure ;
  rdfs:label "Diffraction Grating"@en ;
  rdfs:comment "Diffraction Grating is an Optical Instrument with a periodic structure that is designed to split and defract a beam of light into several beams travelling in different directions."@en .

cco:ont00001179 rdf:type owl:Class ;
  rdfs:subClassOf :InformationMediumArtifact ;
  rdfs:label "Digital Storage Device"@en ;
  rdfs:comment "Digital Storage Device is an Information Medium Artifact that is designed to bear some Information Content Entity by means of recording that information in digital (binary) format."@en .

cco:ont00001304 rdf:type owl:Class ;
  rdfs:subClassOf :QualitySpecification ;
  rdfs:label "Dimension Specification"@en ;
  rdfs:comment "Dimension Specification is a Quality Specification that prescribes some Size Quality."@en .

cco:ont00000790 rdf:type owl:Class ;
  rdfs:subClassOf :ElectricalPowerSource ,
        [ rdf:type owl:Restriction ;
      owl:onProperty :bearer_of ;
      owl:someValuesFrom cco:ont00000994
    ] ;
  rdfs:label "Direct Current Power Source"@en ;
  rdfs:comment "Direct Current Power Source is an Electrical Power Source that is designed to transfer electrical power in the form of direct current."@en .

cco:ont00000965 rdf:type owl:Class ;
  rdfs:subClassOf :InformationContentEntity ;
  rdfs:label "Directive Information Content Entity"@en ;
  rdfs:comment "Directive Information Content Entity is an Information Content Entity that consists of a set of propositions or images (as in the case of a blueprint) that prescribe some Entity."@en .

cco:ont00001223 rdf:type owl:Class ;
  rdfs:subClassOf :RadioReceiver ;
  rdfs:label "Dish Receiver"@en ;
  rdfs:comment "Dish Receiver is a Radio Receiver that uses a Parabolic (or Dish) Antenna to intercept radio signals."@en .

cco:ont00000028 rdf:type owl:Class ;
  rdfs:subClassOf :Prism ;
  rdfs:label "Dispersive Prism"@en ;
  rdfs:comment "Dispersive Prism is a Prism designed to break up a beam of light entering the Prism into its constituent spectral colors by leveraging the refractive index of light based on its Frequency."@en .

cco:ont00000716 rdf:type owl:Class ;
  rdfs:subClassOf :ElectricalPowerSource ,
        [ rdf:type owl:Restriction ;
      owl:onProperty :bearer_of ;
      owl:someValuesFrom cco:ont00000994
    ] ;
  rdfs:label "Electric Battery"@en ;
  rdfs:comment "Electric Battery is an Electrical Power Source that is designed to produce electric power by converting chemical energy to electrical energy."@en .

cco:ont00001025 rdf:type owl:Class ;
  rdfs:subClassOf :ElectricalPowerSource ;
  rdfs:label "Electric Generator"@en ;
  rdfs:comment "Electric Generator is an Electrical Power Source that is designed to convert mechanical energy to electrical energy for use in an external circuit."@en .

cco:ont00000952 rdf:type owl:Class ;
  rdfs:subClassOf :Engine ,
        [ rdf:type owl:Restriction ;
      owl:onProperty :bearer_of ;
      owl:someValuesFrom cco:ont00000098
    ] ;
  rdfs:label "Electric Motor"@en ;
  rdfs:comment "Electric Motor is an Engine that is designed to convert electrical energy into mechanical energy."@en .

cco:ont00001049 rdf:type owl:Class ;
  rdfs:subClassOf :PowerSource ;
  rdfs:label "Electrical Power Source"@en ;
  rdfs:comment "Electrical Power Source is a Power Source that is designed to generate, control, and transfer power in the form of electrical energy."@en .

cco:ont00000413 rdf:type owl:Class ;
  rdfs:subClassOf :Microscope ;
  rdfs:label "Electron Microscope"@en ;
  rdfs:comment "Electron Microscope is a Microscope that is designed to use a beam of accelerated electrons to illuminate the target and produce a significantly enlarged image of the Object."@en .

cco:ont00000347 rdf:type owl:Class ;
  rdfs:subClassOf :Bond ;
  rdfs:label "Electronic Bond"@en ;
  rdfs:comment "Electronic Bond is a Bond that consists of Bytes."@en .

cco:ont00001382 rdf:type owl:Class ;
  rdfs:subClassOf :PortionofCash ;
  rdfs:label "Electronic Cash"@en ;
  rdfs:comment "Electronic Cash is a Portion of Cash that consists of Bytes."@en .

cco:ont00000025 rdf:type owl:Class ;
  rdfs:subClassOf :Stock ;
  rdfs:label "Electronic Stock"@en ;
  rdfs:comment "Electronic Stock is a Stock that consists of Bytes."@en .

cco:ont00000906 rdf:type owl:Class ;
  rdfs:subClassOf :TelecommunicationInstrument ;
  rdfs:label "Email Box"@en ;
  rdfs:comment "Email Box is a Telecommunication Instrument that is designed to be the delivery destination of Email Messages that are addressed to the corresponding Email Address."@en .

cco:ont00000909 rdf:type owl:Class ;
  rdfs:subClassOf :ElectricalPowerSource ,
        [ rdf:type owl:Restriction ;
      owl:onProperty :bearer_of ;
      owl:someValuesFrom cco:ont00000994
    ] ;
  rdfs:label "Emergency AC/DC Power Source"@en ;
  rdfs:comment "Emergency AC/DC Power Source is an Electrical Power Source that is designed to provide electrical power in an emergency situation by means of both alternating current and direct current."@en .

cco:ont00000285 rdf:type owl:Class ;
  rdfs:subClassOf :RadioTransmitter ,
        [ rdf:type owl:Restriction ;
      owl:onProperty :bearer_of ;
      owl:someValuesFrom cco:ont00000317
    ] ;
  rdfs:label "Emergency Locator Transmitter"@en ;
  rdfs:comment "Emergency Locator Transmitter is a Radio Transmitter that is designed to signal distress and provide positional data for the entity it is located on."@en .

cco:ont00000210 rdf:type owl:Class ;
  rdfs:subClassOf :MaterialArtifact ;
  rdfs:label "Engine"@en ;
  rdfs:comment "Engine is a Material Artifact that is designed to convert one form of energy into mechanical energy."@en .

cco:ont00000453 rdf:type owl:Class ;
  rdfs:subClassOf :MaterialArtifact ,
        [ rdf:type owl:Restriction ;
      owl:onProperty :bearer_of ;
      owl:someValuesFrom cco:ont00000679
    ] ;
  rdfs:label "Environment Control System"@en ;
  rdfs:comment "Environment Control System is a Material Artifact that is designed to control the temperature, air quality, or other feature of a Site that is relevant to the comfort or operation of entities located within that Site."@en .

cco:ont00001018 rdf:type owl:Class ;
  rdfs:subClassOf :CoolingSystem ;
  rdfs:label "Equipment Cooling System"@en ;
  rdfs:comment "Equipment Cooling System is a Cooling System that is designed to cool some piece of equipment."@en .

cco:ont00001042 rdf:type owl:Class ;
  rdfs:subClassOf :MaterialArtifact ,
        [ rdf:type owl:Restriction ;
      owl:onProperty :bearer_of ;
      owl:someValuesFrom cco:ont00000480
    ] ;
  rdfs:label "Equipment Mount"@en ;
  rdfs:comment "Equipment Mount is a Material Artifact that is designed to support an Artifact."@en .

cco:ont00000734 rdf:type owl:Class ;
  rdfs:subClassOf :ExplosiveMine ;
  rdfs:label "Explosive Land Mine"@en ;
  rdfs:comment "Explosive Land Mine is an Explosive Mine that is designed to be concealed under or on the ground."@en .

cco:ont00002066 rdf:type owl:Class ;
  rdfs:subClassOf :ExplosiveWeapon ;
  rdfs:label "Explosive Mine"@en ;
  rdfs:comment "Explosive Mine is an Explosive Weapon that is designed to be concealed and to detonate as its target passes near it."@en .

cco:ont00002067 rdf:type owl:Class ;
  rdfs:subClassOf :ExplosiveMine ;
  rdfs:label "Explosive Naval Mine"@en ;
  rdfs:comment "Explosive Naval Mine is an Explosive Mine that is designed to be concealed on or under water."@en .

cco:ont00000552 rdf:type owl:Class ;
  rdfs:subClassOf :Weapon ;
  rdfs:label "Explosive Weapon"@en ;
  rdfs:comment "Explosive Weapon is a Weapon that is designed to inflict harm, damage, or incapacity by means of a violent release of energy caused by the exothermic reaction of an explosive material."@en .

cco:ont00000431 rdf:type owl:Class ;
  rdfs:subClassOf :CombustionEngine ;
  rdfs:label "External Combustion Engine"@en ;
  rdfs:comment "External Combustion Engine is a Combustion Engine that is designed to have an external Combustion Chamber where portions of Fuel and Oxidizer mixture are burned to generate thermal energy to heat the working fluid, which transfers energy to the Engine where it is converted into mechanical energy."@en .

cco:ont00000681 rdf:type owl:Class ;
  rdfs:subClassOf :LightingSystem ;
  rdfs:label "External Navigation Lighting System"@en ;
  rdfs:comment "External Navigation Lighting System is a Lighting System that is designed to be attached to some Vehicle and to emit colored light in order to signal that Vehicle's position, heading, and status."@en .

cco:ont00000192 rdf:type owl:Class ;
  rdfs:subClassOf :MaterialArtifact ;
  rdfs:label "Facility"@en ;
  rdfs:comment "Facility is a Material Artifact that is designed as a building or campus dedicated to some specific purpose."@en .

cco:ont00000338 rdf:type owl:Class ;
  rdfs:subClassOf :FluidControlArtifact ;
  rdfs:label "Fan"@en ;
  rdfs:comment "Fan is a Fluid Control Artifact that consists of a rotating arrangement of vanes or blades that are designed to act on a portion of fluid to create flow within it."@en .

cco:ont00000348 rdf:type owl:Class ;
  rdfs:subClassOf :MaterialArtifact ;
  rdfs:label "Filter"@en ;
  rdfs:comment "Filter is a Material Artifact that bears a Filter Function."@en .

cco:ont00000537 rdf:type owl:Class ;
  rdfs:subClassOf :MaterialArtifact ;
  rdfs:label "Financial Instrument"@en ;
  rdfs:comment "Financial Instrument is a Material Artifact that is designed to be a tradeable asset and that is legally sanctioned."@en .

cco:ont00000088 rdf:type owl:Class ;
  rdfs:subClassOf :ProjectileLauncher ;
  rdfs:label "Firearm"@en ;
  rdfs:comment "Firearm is a Projectile Launcher that is designed to launch Bullets or Cartridges."@en .

cco:ont00000147 rdf:type owl:Class ;
  rdfs:subClassOf :RadioTransponder ;
  rdfs:label "Flight Transponder"@en ;
  rdfs:comment "Flight Transponder is a Radio Transponder that is designed to produce a specified response (typically for identification, location, or status update purposes) when it receives a radio-frequency interrogation."@en .

cco:ont00000047 rdf:type owl:Class ;
  rdfs:subClassOf :Valve ;
  rdfs:label "Flow Control Valve"@en ;
  rdfs:comment "Flow Control Valve is a Valve that is designed to regulate the flow or Pressure of a fluid."@en .

cco:ont00000256 rdf:type owl:Class ;
  rdfs:subClassOf :MaterialArtifact ;
  rdfs:label "Fluid Control Artifact"@en ;
  rdfs:comment "Fluid Control Artifact is a Material Artifact that is designed to manipulate the flow of a fluid (i.e. a liquid or a gas)."@en .

cco:ont00001140 rdf:type owl:Class ;
  rdfs:subClassOf :MaterialArtifact ;
  rdfs:label "Flywheel"@en ;
  rdfs:comment "Flywheel is a Material Artifact that is designed to store rotational energy such that it has a significant moment of inertia which enables it to resist changes in rotational speed."@en .

cco:ont00001355 rdf:type owl:Class ;
  rdfs:subClassOf :TrainCar ;
  rdfs:label "Freight Train Car"@en ;
  rdfs:comment "Freight Train Car is a Train Car that is designed to transport cargo."@en .

cco:ont00000477 rdf:type owl:Class ;
  rdfs:subClassOf :ElectricalPowerSource ;
  rdfs:label "Fuel Cell"@en ;
  rdfs:comment "Fuel Cell is an Electrical Power Source that consists in part of an anode, a cathode, and an electrolyte; converts chemical energy from a fuel into electricity through a chemical reaction of positively charged hydrogen ions with an oxidizing agent (typically oxygen); and, if given a continuous source of fuel and oxidizing agent, can continuously produce electricity."@en .

cco:ont00001060 rdf:type owl:Class ;
  rdfs:subClassOf :MaterialArtifact ;
  rdfs:label "Fuel System"@en ;
  rdfs:comment "Fuel System is a Material Artifact that is designed to pump, manage, and deliver some Portion of Fuel to the Propulsion System and Auxiliary Power Unit of some Vehicle."@en .

cco:ont00000691 rdf:type owl:Class ;
  rdfs:subClassOf :Container ;
  rdfs:label "Fuel Tank"@en ;
  rdfs:comment "Fuel Tank is a Container that is designed to store a Portion of Fuel."@en .

cco:ont00000963 rdf:type owl:Class ;
  rdfs:subClassOf :FluidControlArtifact ;
  rdfs:label "Fuel Transfer System"@en ;
  rdfs:comment "Fuel Transfer System is a Fluid Control Artifact that is designed to facilitate the transfer of some Portion of Fuel from the Fuel Tank for use in some Engine."@en .

cco:ont00000793 rdf:type owl:Class ;
  rdfs:subClassOf :FluidControlArtifact ;
  rdfs:label "Fuel Ventilation System"@en ;
  rdfs:comment "Fuel Ventilation System is a Fluid Control Artifact that is designed to allow air into the Fuel Tank to take the place of burned fuel."@en .

cco:ont00001034 rdf:type owl:Class ;
  rdfs:subClassOf :VideoCamera ;
  rdfs:label "Full Motion Video Camera"@en ;
  rdfs:comment "Full Motion Video Camera is a Video Camera that is designed to capture and record images of sufficiently high quality and in rapid enough succession that the resulting video supports smooth playback."@en .

cco:ont00000526 rdf:type owl:Class ;
  rdfs:subClassOf :Telescope ;
  rdfs:label "Gamma-ray Telescope"@en ;
  rdfs:comment "Gamma-ray Telescope is a Telescope that is designed to aid in the observation of spatially distant Objects by means of collecting and focusing Gamma-rays to form an enhanced image of the Object."@en .

cco:ont00000333 rdf:type owl:Class ;
  rdfs:subClassOf :InternalCombustionEngine ;
  rdfs:label "Gas Turbine"@en ;
  rdfs:comment "Gas Turbine is an Internal Combustion Engine that has a rotating compressor and a turbine and is designed to operate utilizing continous Combustion to produce Thrust, either directly via exhaust or indirectly via a prop."@en .

cco:ont00000153 rdf:type owl:Class ;
  rdfs:subClassOf :ControlSystem ;
  rdfs:label "Generator Control Unit"@en ;
  rdfs:comment "Generator Control Unit is a Control System that is designed to regulate the voltage of some Electrical Power Source."@en .

cco:ont00001316 rdf:type owl:Class ;
  rdfs:subClassOf :EquipmentMount ;
  rdfs:label "Gimbal"@en ;
  rdfs:comment "Gimbal is an Equipment Mount that consists of a pivoted support that allows an Artifact to Rotate about one or more Axes."@en .

cco:ont00000310 rdf:type owl:Class ;
  rdfs:subClassOf :ExplosiveWeapon ;
  rdfs:label "Grenade"@en ;
  rdfs:comment "Grenade is an Explosive Weapon that is designed to be relatively small and to be thrown by hand."@en .

cco:ont00000053 rdf:type owl:Class ;
  rdfs:subClassOf :GroundVehicle ,
        [ rdf:type owl:Restriction ;
      owl:onProperty :bearer_of ;
      owl:someValuesFrom cco:ont00000994
    ] ;
  rdfs:label "Ground Motor Vehicle"@en ;
  rdfs:comment "Ground Motor Vehicle is a Ground Vehicle that is designed to receive its motive power from an Engine and is not designed to travel on rails."@en .

cco:ont00000618 rdf:type owl:Class ;
  rdfs:subClassOf :Vehicle ;
  rdfs:label "Ground Vehicle"@en ;
  rdfs:comment "Ground Vehicle is a Vehicle that is designed to convey passengers, cargo, or equipment from one location to another by some form of ground travel."@en .

cco:ont00000156 rdf:type owl:Class ;
  rdfs:subClassOf :Firearm ;
  rdfs:label "Hand Gun"@en ;
  rdfs:comment "Hand Gun is a Firearm that is designed to have a relatively short barrel and to be held in one or two hands and to be fired without being braced against the shoulder."@en .

cco:ont00000266 rdf:type owl:Class ;
  rdfs:subClassOf :MedicalArtifact ;
  rdfs:label "Hearing Aid"@en ;
  rdfs:comment "Hearing Aid is a Medical Artifact that is designed to improve hearing for its user."@en .

cco:ont00000638 rdf:type owl:Class ;
  rdfs:subClassOf :Engine ;
  rdfs:label "Heat Engine"@en ;
  rdfs:comment "Heat Engine is an Engine that is designed to convert thermal energy into mechanical energy."@en .

cco:ont00000243 rdf:type owl:Class ;
  rdfs:label "Heat Sink"@en ;
  rdfs:comment "A Material Artifact that is designed to passively dissipate heat from components or systems in order to control temperature."@en .

cco:ont00000849 rdf:type owl:Class ;
  rdfs:subClassOf :EnvironmentControlSystem ;
  rdfs:label "Heating System"@en ;
  rdfs:comment "Heating System is an Environment Control System that is designed to heat the air or objects in a Site."@en .

cco:ont00001077 rdf:type owl:Class ;
  rdfs:subClassOf :MountedGun ;
  rdfs:label "Heavy Machine Gun"@en ;
  rdfs:comment "Heavy Machine Gun is a Mounted Gun that is designed to fire ammunition greater than .50 caliber or 12.7mm ammunition in quick succession from an ammunition belt, and which typically weighs more than 30lbs."@en .

cco:ont00001054 rdf:type owl:Class ;
  rdfs:subClassOf :WireAntenna ;
  rdfs:label "Helical Antenna"@en ;
  rdfs:comment "Helical Antenna is a Wire Antenna that consists of a conducting wire wound in the form of a helix that is typically mounted over a ground plane with a feed line connected between the bottom of the helix and the ground plane."@en .

cco:ont00000888 rdf:type owl:Class ;
  rdfs:label "High Frequency Communication Instrument"@en ;
  rdfs:comment "A Radio Communication Instrument that is designed to transmit and/or receive radio signals in the high-frequency (HF) band."@en .

cco:ont00000646 rdf:type owl:Class ;
  rdfs:subClassOf :Road ,
        [ rdf:type owl:Restriction ;
      owl:onProperty :bearer_of ;
      owl:someValuesFrom cco:ont00000650
    ] ;
  rdfs:label "Highway"@en ;
  rdfs:comment "Highway is a Road that is designed to enable Ground Vehicles to travel between relatively major destinations."@en .

cco:ont00000956 rdf:type owl:Class ;
  rdfs:subClassOf :RoadJunction ,
        [ rdf:type owl:Restriction ;
      owl:onProperty :bearer_of ;
      owl:someValuesFrom cco:ont00000650
    ] ;
  rdfs:label "Highway Interchange"@en ;
  rdfs:comment "Highway Interchange is a Road Junction that is designed to enable Ground Vehicles to exit one or more Highways and enter another Highway without directly crossing any other traffic stream."@en .

cco:ont00000306 rdf:type owl:Class ;
  rdfs:subClassOf :MachineBearing ;
  rdfs:label "Hinge"@en ;
  rdfs:comment "Hinge is a Machine Bearing that is designed to limit the angle of Rotation between two solid objects."@en .

cco:ont00000714 rdf:type owl:Class ;
  rdfs:subClassOf :RadioAntenna ;
  rdfs:label "Horn Antenna"@en ;
  rdfs:comment "Horn Antenna is a Radio Antenna that consists of a flaring metal waveguide shaped like a horn to direct radio waves in a beam and can be used on its own or as a feeder for larger antenna structures, such as Parabolic Antennas."@en .

cco:ont00001270 rdf:type owl:Class ;
  rdfs:subClassOf :Cannon ;
  rdfs:label "Howitzer"@en ;
  rdfs:comment "Howitzer is a Cannon that is designed to have a relatively short barrel and to use relatively small propellant charges to propel projectiles in relatively high trajectories with a steep angle of descent."@en .

cco:ont00000264 rdf:type owl:Class ;
  rdfs:subClassOf :Container ;
  rdfs:label "Hydraulic Fluid Reservoir"@en ;
  rdfs:comment "Hydraulic Fluid Reservoir is a Container that is designed to store some hydraulic fluid for use in some Hyrdraulic Power Source."@en .

cco:ont00000777 rdf:type owl:Class ;
  rdfs:subClassOf :PhysicallyPoweredEngine ;
  rdfs:label "Hydraulic Motor"@en ;
  rdfs:comment "Hydraulic Motor is a Physically Powered Engine that converts hydraulic pressure and flow into torque and angular displacement."@en .

cco:ont00001157 rdf:type owl:Class ;
  rdfs:subClassOf :PowerSource ;
  rdfs:label "Hydraulic Power Source"@en ;
  rdfs:comment "Hydraulic Power Source is a Power Source that is designed to generate, control, or transmit power by means of pressurized liquid."@en .

cco:ont00000730 rdf:type owl:Class ;
  rdfs:label "Hydraulic Power Transfer Unit"@en ;
  rdfs:comment "A Material Artifact that is designed to transfer hydraulic power between hydraulic systems; in aircraft, it can transfer power between independent systems when one has failed or is offline."@en .

cco:ont00001282 rdf:type owl:Class ;
  rdfs:subClassOf :Valve ;
  rdfs:label "Hydraulic Valve"@en ;
  rdfs:comment "Hydraulic Valve is a Valve that is designed to regulate, direct, or control the flow of a liquid by opening, closing, or partially obstructing various passageways."@en .

cco:ont00000878 rdf:type owl:Class ;
  rdfs:subClassOf :RadioTransponder ;
  rdfs:label "Identification Friend or Foe Transponder"@en ;
  rdfs:comment "Identification Friend or Foe Transponder is a Radio Transponder that is designed to automatically transmit a predefined signal in response to receiving an appropriate interrogation signal such that the entity it is located on can be positively identified as friendly."@en .

cco:ont00000742 rdf:type owl:Class ;
  rdfs:subClassOf :MaterialArtifact ;
  rdfs:label "Ignition System"@en ;
  rdfs:comment "Ignition System is a Material Artifact that is designed to produce an Ignition process."@en .

cco:ont00000771 rdf:type owl:Class ;
  rdfs:subClassOf :MaterialArtifact ;
  rdfs:label "Imaging Instrument"@en ;
  rdfs:comment "Imaging Instrument is a Material Artifact that is designed to produce images (visual representations) of an entity."@en .

cco:ont00000858 rdf:type owl:Class ;
  rdfs:subClassOf :ExplosiveWeapon ;
  rdfs:label "Improvised Explosive Device"@en ;
  rdfs:comment "Improvised Explosive Device is an Explosive Weapon that is designed to be used in non-conventional military action."@en .

cco:ont00000145 rdf:type owl:Class ;
  rdfs:subClassOf :Weapon ;
  rdfs:label "Incendiary Weapon"@en ;
  rdfs:comment "Incendiary Weapon is a Weapon that is designed to inflict harm, damage, or incapacity by means of starting a fire."@en .

cco:ont00000287 rdf:type owl:Class ;
  rdfs:subClassOf :NavigationSystem ;
  rdfs:label "Inertial Navigation System"@en ;
  rdfs:comment "Inertial Navigation System is a Navigation System that is designed to continuously calculate via dead reckoning the position, orientation, and velocity of a moving object without the need for external references."@en .

cco:ont00001342 rdf:type owl:Class ;
  rdfs:subClassOf :ArmoredFightingVehicle ;
  rdfs:label "Infantry Fighting Vehicle"@en ;
  rdfs:comment "Infantry Fighting Vehicle is an Armored Fighting Vehicle that is designed to carry infantry into battle and to provide fire support for them."@en .

cco:ont00000798 rdf:type owl:Class ;
  rdfs:subClassOf :MaterialArtifact ;
  rdfs:label "Information Bearing Artifact"@en ;
  rdfs:comment "Information Bearing Artifact is a Material Artifact that carries an Information Content Entity and is designed to do so using a particular format or structure."@en .

cco:ont00000253 rdf:type owl:Class ;
  rdfs:subClassOf :Objectupon ;
  rdfs:label "Information Bearing Entity"@en ;
  rdfs:comment "Information Bearing Entity is an Object upon that an Information Content Entity generically depends."@en .

cco:ont00000958 rdf:type owl:Class ;
  rdfs:subClassOf :GenericallyDependentContinuant ;
  rdfs:label "Information Content Entity"@en ;
  rdfs:comment "Information Content Entity is a Generically Dependent Continuant that generically depends on some Information Bearing Entity and stands in relation of aboutness to some Entity."@en .

cco:ont00000893 rdf:type owl:Class ;
  rdfs:subClassOf :MaterialArtifact ;
  rdfs:label "Information Medium Artifact"@en ;
  rdfs:comment "Information Medium Artifact is a Material Artifact that is designed to have some Information Bearing Artifact as part."@en .

cco:ont00000117 rdf:type owl:Class ;
  rdfs:subClassOf :MaterialArtifact ;
  rdfs:label "Information Processing Artifact"@en ;
  rdfs:comment "Information Processing Artifact is a Material Artifact that is designed to use algorithms to transform some Information Content Entity into another Information Content Entity."@en .

cco:ont00000617 rdf:type owl:Class ;
  rdfs:subClassOf :Camera ;
  rdfs:label "Infrared Camera"@en ;
  rdfs:comment "Infrared Camera is a Camera that is designed to form and record an image generated from infrared radiation."@en .

cco:ont00000090 rdf:type owl:Class ;
  rdfs:subClassOf :Telescope ;
  rdfs:label "Infrared Telescope"@en ;
  rdfs:comment "Infrared Telescope is a Telescope that is designed to aid in the observation of spatially distant Objects by means of collecting and focusing infrared light to form an enhanced image of the Object."@en .

cco:ont00000627 rdf:type owl:Class ;
  rdfs:subClassOf :MaterialEntity ;
  rdfs:label "Infrastructure Element"@en ;
  rdfs:comment "Infrastructure Element is a Material Entity that bears an Infrastructure Role."@en .

cco:ont00001141 rdf:type owl:Class ;
  rdfs:subClassOf :Role ;
  rdfs:label "Infrastructure Role"@en ;
  rdfs:comment "Infrastructure Role is a Role that inheres in the bearer of a Disposition and has been assigned to an Infrastructure System such that the realization of that Disposition is sometimes part of the functioning of the Infrastructure System."@en .

cco:ont00000870 rdf:type owl:Class ;
  rdfs:subClassOf :MaterialEntity ;
  rdfs:label "Infrastructure System"@en ;
  rdfs:comment "Infrastructure System is a Material Entity that is composed of elements bearing Infrastructure Roles and is by itself sufficient to provide a planned service or benefit to some organization that maintains its elements."@en .

cco:ont00000303 rdf:type owl:Class ;
  rdfs:subClassOf :CommunicationSystem ;
  rdfs:label "Intercommunication System"@en ;
  rdfs:comment "Intercommunication System is a Communication System that is designed to enable some Act of Communication between end points within a building, small collection of buildings, or within a small area of service."@en .

cco:ont00001250 rdf:type owl:Class ;
  rdfs:subClassOf :LightingSystem ;
  rdfs:label "Interior Lighting System"@en ;
  rdfs:comment "Interior Lighting System is a Lighting System that is designed to emit light within the interior of some area."@en .

cco:ont00000394 rdf:type owl:Class ;
  rdfs:subClassOf :CombustionEngine ;
  rdfs:label "Internal Combustion Engine"@en ;
  rdfs:comment "Internal Combustion Engine is a Combustion Engine that is designed to have an internal Combustion Chamber where portions of Fuel and Oxidizer mixture are burned to generate thermal energy that is then converted into mechanical energy."@en .

cco:ont00000334 rdf:type owl:Class ;
  rdfs:subClassOf :IntercommunicationSystem ;
  rdfs:label "Interphone"@en ;
  rdfs:comment "Interphone is an Intercommunication System that that is designed to facilitate some Act of Communication between agents by means of audio messages."@en .

cco:ont00000533 rdf:type owl:Class ;
  rdfs:subClassOf :ReactionEngine ;
  rdfs:label "Jet Engine"@en ;
  rdfs:comment "Jet Engine is a Reaction Engine that discharges a fast moving jet that generates Thrust by jet propulsion."@en .

cco:ont00001326 rdf:type owl:Class ;
  rdfs:subClassOf :TransportationArtifact ;
  rdfs:label "Land Transportation Artifact"@en ;
  rdfs:comment "Land Transportation Artifact is a Transportation Artifact that facilitates the movement of Agents and Vehicles via land."@en .

cco:ont00000933 rdf:type owl:Class ;
  rdfs:subClassOf :Telephone ;
  rdfs:label "Landline Telephone"@en ;
  rdfs:comment "Landline Telephone is a Telephone that is connected to a Telephone Network through a pair of wires."@en .

cco:ont00000167 rdf:type owl:Class ;
  rdfs:subClassOf :RocketLauncher ;
  rdfs:label "Large-Scale Rocket Launcher"@en ;
  rdfs:comment "Large-Scale Rocket Launcher is a Rocket Launcher that is designed to contain multiple Rocket Launchers."@en .

cco:ont00001067 rdf:type owl:Class ;
  rdfs:subClassOf :MaterialArtifact ;
  rdfs:label "Laser"@en ;
  rdfs:comment "Laser is a Material Artifact that is designed to emit light coherently through a process of optical amplification based on the stimulated emission of electromagnetic radiation."@en .

cco:ont00001321 rdf:type owl:Class ;
  rdfs:subClassOf :SecondaryCellElectricBattery ;
  rdfs:label "Lead Acid Electric Battery"@en ;
  rdfs:comment "Lead Acid Electric Battery is a Secondary Cell Electric Battery that has a lead anode and lead oxide cathode."@en .

cco:ont00001346 rdf:type owl:Class ;
  rdfs:subClassOf :MaterialArtifact ;
  rdfs:label "Legal Instrument"@en ;
  rdfs:comment "Legal Instrument is a Material Artifact that is designed as a formally executed written document that can be formally attributed to its author, records and formally expresses a legally enforceable act, process, or contractual duty, obligation, or right, and therefore evidences that act, process, or agreement."@en .

cco:ont00000851 rdf:type owl:Class ;
  rdfs:subClassOf :LongGun ;
  rdfs:label "Light Machine Gun"@en ;
  rdfs:comment "Light Machine Gun is a Long Gun that is designed to fire bullets in quick succession from an ammunition belt or magazine and to be employed by an individual soldier, with or without assistance, and typically weighing 9-22 lbs."@en .

cco:ont00000236 rdf:type owl:Class ;
  rdfs:subClassOf :MaterialArtifact ;
  rdfs:label "Lighting System"@en ;
  rdfs:comment "Lighting System is a Material Artifact that is designed to emit light within some area."@en .

cco:ont00000158 rdf:type owl:Class ;
  rdfs:subClassOf :SecondaryCellElectricBattery ;
  rdfs:label "Lithium-ion Electric Battery"@en ;
  rdfs:comment "Lithium-ion Electric Battery is a Secondary Cell Electric Battery that produces electricity when lithium ions move from anode to cathode."@en .

cco:ont00000775 rdf:type owl:Class ;
  rdfs:subClassOf :RailTransportVehicle ;
  rdfs:label "Locomotive"@en ;
  rdfs:comment "Locomotive is a Rail Transport Vehicle that is designed to provide the motive power for a Train."@en .

cco:ont00001104 rdf:type owl:Class ;
  rdfs:subClassOf :Firearm ;
  rdfs:label "Long Gun"@en ;
  rdfs:comment "Long Gun is a Firearm that is designed to have a longer barrel than a Hand Gun and to be fired while braced against the shoulder."@en .

cco:ont00000767 rdf:type owl:Class ;
  rdfs:subClassOf :MaterialArtifact ;
  rdfs:label "Lubrication System"@en ;
  rdfs:comment "Lubrication System is a Material Artifact that is designed to contain, transfer, and regulate the flow of lubricant to multiple locations in an Artifact."@en .

cco:ont00001370 rdf:type owl:Class ;
  rdfs:subClassOf :MaterialArtifact ,
        [ rdf:type owl:Restriction ;
      owl:onProperty :bearer_of ;
      owl:someValuesFrom cco:ont00001155
    ] ;
  rdfs:label "Machine Bearing"@en ;
  rdfs:comment "Machine Bearing is a Material Artifact that is designed to constrain relative motion to only desired motion and reduces friction between moving parts."@en .

cco:ont00000160 rdf:type owl:Class ;
  rdfs:subClassOf :Tool ;
  rdfs:label "Manual Tool"@en ;
  rdfs:comment "Manual Tool is a Tool that is designed to be powered by manual labor rather than by an engine."@en .

cco:ont00000693 rdf:type owl:Class ;
  rdfs:subClassOf :QualitySpecification ;
  rdfs:label "Mass Specification"@en ;
  rdfs:comment "Mass Specification is a Quality Specification that prescribes the Amount of Mass that a Material Entity should have."@en .

cco:ont00000995 rdf:type owl:Class ;
  rdfs:subClassOf :MaterialEntity ;
  rdfs:label "Material Artifact"@en ;
  rdfs:comment "Material Artifact is a Material Entity that was designed by some Agent to realize a certain Function."@en .

cco:ont00000470 rdf:type owl:Class ;
  rdfs:subClassOf :MaterialCopyofaCertificate ;
  rdfs:label "Material Copy of a Academic Degree"@en ;
  rdfs:comment "Material Copy of a Academic Degree is a Material Copy of a Certificate that is issued by an Educational Organization to a Person to indicate that the Person has satisfactorily completed a course of study, or as an honorary recognition of the Person's achievement."@en .

cco:ont00000014 rdf:type owl:Class ;
  rdfs:label "Material Copy of a Aztec Code"@en ;
  rdfs:comment "Material Copy of a Aztec Code is a Material Copy of a Two-Dimensional Barcode that is used by the transportation industry to scan tickets."@en .

cco:ont00001064 rdf:type owl:Class ;
  rdfs:subClassOf :InformationBearingArtifact ;
  rdfs:label "Material Copy of a Barcode"@en ;
  rdfs:comment "Material Copy of a Barcode is an Information Bearing Artifact that is designed to carry one or more geometric shapes that concretize some Directive Information Content Entity."@en .

cco:ont00000064 rdf:type owl:Class ;
  rdfs:subClassOf :MaterialCopyofaDocument ;
  rdfs:label "Material Copy of a Book"@en ;
  rdfs:comment "Material Copy of a Book is a Material Copy of a Document that is designed to carry some specific Information Content Entity by means of ink, paper, parchment, or other materials fastened together to hinge at one side."@en .

cco:ont00000189 rdf:type owl:Class ;
  rdfs:subClassOf :InformationBearingArtifact ;
  rdfs:label "Material Copy of a Certificate"@en ;
  rdfs:comment "Material Copy of a Certificate is an Information Bearing Artifact that bears an Information Content Entity which attests to certain demonstrated characteristics of an Object, Person, or Organization."@en .

cco:ont00000743 rdf:type owl:Class ;
  rdfs:subClassOf :MaterialCopyofanImage ;
  rdfs:label "Material Copy of a Chart"@en ;
  rdfs:comment "Material Copy of a Chart is a Material Copy of an Image that is designed to carry some Representational Information Content Entity that is prescribed by some canonical visual format."@en .

cco:ont00000429 rdf:type owl:Class ;
  rdfs:label "Material Copy of a Codabar Barcode"@en ;
  rdfs:comment "Material Copy of a Codabar Barcode is a Material Copy of a One-Dimensional Barcode that consists of numbers 0-9 and the characters -$:/.+ and is used by logistics and healthcare professionals."@en .

cco:ont00001264 rdf:type owl:Class ;
  rdfs:label "Material Copy of a Code 128 Barcode"@en ;
  rdfs:comment "Material Copy of a Code 128 Barcode is a Material Copy of a One-Dimensional Barcode that consists of up to 128 ASCII characters and is used primarily in supply chains."@en .

cco:ont00001260 rdf:type owl:Class ;
  rdfs:label "Material Copy of a Code 39 Barcode"@en ;
  rdfs:comment "Material Copy of a Code 39 Barcode is a Material Copy of a One-Dimensional Barcode that consists of 39 characters that are numbers 0-9, capital letters A-Z, or the symbols -.$/+% and space and is used primarily in automotive and defense industries."@en .

cco:ont00000582 rdf:type owl:Class ;
  rdfs:label "Material Copy of a Code 93 Barcode"@en ;
  rdfs:comment "Material Copy of a Code 93 Barcode is a Material Copy of a One-Dimensional Barcode that consists of up to 93 ASCII characters and is used in logistics to identify packages in retail inventory, lable electornic components, and provide supplementary delivery information."@en .

cco:ont00000493 rdf:type owl:Class ;
  rdfs:subClassOf :MaterialCopyofaList ;
  rdfs:label "Material Copy of a Code List"@en ;
  rdfs:comment "Material Copy of a Code List is a Material Copy of a List that contains an ordered sequence of Information Bearing Entities that carry Code Identifiers."@en .

cco:ont00000242 rdf:type owl:Class ;
  rdfs:label "Material Copy of a Data Matrix Code"@en ;
  rdfs:comment "Material Copy of a Data Matrix Code is a Material Copy of a Two-Dimensional Barcode that consists of cells arranged in rectangular patterns and is used for marking small items in logistics and operations."@en .

cco:ont00000756 rdf:type owl:Class ;
  rdfs:subClassOf :InformationBearingArtifact ;
  rdfs:label "Material Copy of a Database"@en ;
  rdfs:comment "Material Copy of a Database is an Information Bearing Artifact that is designed to carry some set of specific Information Content Entities and to be rapidly searchable and retrievable."@en .

cco:ont00001298 rdf:type owl:Class ;
  rdfs:subClassOf :InformationBearingArtifact ;
  rdfs:label "Material Copy of a Document"@en ;
  rdfs:comment "Material Copy of a Document is an Information Bearing Artifact that is designed to carry some specific Information Content Entity in a series of paragraphs of text or diagrams in the form of physical pieces of paper or an electronic word processor file."@en .

cco:ont00001243 rdf:type owl:Class ;
  rdfs:subClassOf :InformationBearingEntity ;
  rdfs:label "Material Copy of a Document Field"@en ;
  rdfs:comment "Material Copy of a Document Field is an Information Bearing Entity that is a part of some document into which carriers of prescribed information can be written or selected."@en .

cco:ont00000966 rdf:type owl:Class ;
  rdfs:label "Material Copy of a EAN Barcode"@en ;
  rdfs:comment "Material Copy of a EAN Barcode is a Material Copy of a One-Dimensional Barcode that consists of 8 or 13 numerical digits and is used to scan consumer goods."@en .

cco:ont00000972 rdf:type owl:Class ;
  rdfs:subClassOf :MaterialCopyofanEANBarcode ;
  rdfs:label "Material Copy of a EAN-13 Barcode"@en ;
  rdfs:comment "Material Copy of a EAN-13 Barcode is a Material Copy of an EAN Barcode that consists of 13 numerical digits and is used to designate products at the point of sale."@en .

cco:ont00001131 rdf:type owl:Class ;
  rdfs:subClassOf :MaterialCopyofanEANBarcode ;
  rdfs:label "Material Copy of a EAN-8 Barcode"@en ;
  rdfs:comment "Material Copy of a EAN-8 Barcode is a Material Copy of an EAN Barcode that consists of 8 numerical digits and is used to designate products at the point of sale."@en .

cco:ont00000640 rdf:type owl:Class ;
  rdfs:subClassOf :MaterialCopyofaMessage ;
  rdfs:label "Material Copy of a Email Message"@en ;
  rdfs:comment "Material Copy of a Email Message is a Material Copy of a Message that is transmitted to the recipient's Email Box."@en .

cco:ont00001119 rdf:type owl:Class ;
  rdfs:subClassOf :MaterialCopyofaDocument ;
  rdfs:label "Material Copy of a Form Document"@en ;
  rdfs:comment "Material Copy of a Form Document is a Material Copy of a Document that has one or more Material Copy of a Document Field as parts in which to write or select prescribed content."@en .

cco:ont00001012 rdf:type owl:Class ;
  rdfs:label "Material Copy of a GS1 DataBar Barcode"@en ;
  rdfs:comment "Material Copy of a GS1 DataBar Barcode is a Material Copy of a One-Dimensional Barcode that consists of 12-14 numerical digits and is used in retail and healthcare."@en .

cco:ont00001156 rdf:type owl:Class ;
  rdfs:subClassOf :InformationBearingArtifact ;
  rdfs:label "Material Copy of a Information Line"@en ;
  rdfs:comment "Material Copy of a Information Line is an Information Bearing Artifact that consists of a single line or row of some larger Information Bearing Artifact of which it is a part."@en .

cco:ont00000597 rdf:type owl:Class ;
  rdfs:subClassOf :InformationBearingArtifact ;
  rdfs:label "Material Copy of a Instrument Display Panel"@en ;
  rdfs:comment "Material Copy of a Instrument Display Panel is an Information Bearing Artifact that is designed to carry information about some Artifact that is derived by the instrumentation Sensors of that Artifact."@en .

cco:ont00001268 rdf:type owl:Class ;
  rdfs:subClassOf :MaterialCopyofanEANBarcode ;
  rdfs:label "Material Copy of a ISBN Barcode"@en ;
  rdfs:comment "Material Copy of a ISBN Barcode is a Material Copy of an EAN Barcode that is used to designate books."@en .

cco:ont00000461 rdf:type owl:Class ;
  rdfs:subClassOf :MaterialCopyofanEANBarcode ;
  rdfs:label "Material Copy of a ISSN Barcode"@en ;
  rdfs:comment "Material Copy of a ISSN Barcode is a Material Copy of an EAN Barcode that is used to designate periodicals."@en .

cco:ont00000602 rdf:type owl:Class ;
  rdfs:label "Material Copy of a ITF Barcode"@en ;
  rdfs:comment "Material Copy of a ITF Barcode is a Material Copy of a One-Dimensional Barcode that consists of an even number of numerical characters and is used primarily in packaging and distribution."@en .

cco:ont00000596 rdf:type owl:Class ;
  rdfs:subClassOf :MaterialCopyofanEANBarcode ;
  rdfs:label "Material Copy of a JAN-13 Barcode"@en ;
  rdfs:comment "Material Copy of a JAN-13 Barcode is a Material Copy of an EAN Barcode that consists of 13 numerical digits and is used primarily in Japan to designate products at the point of sale."@en .

cco:ont00001228 rdf:type owl:Class ;
  rdfs:subClassOf :MaterialCopyofaDocument ;
  rdfs:label "Material Copy of a Journal Article"@en ;
  rdfs:comment "Material Copy of a Journal Article is a Material Copy of a Document that is designed to carry a specific brief composition on a specific topic as part of a Journal Issue."@en .

cco:ont00000799 rdf:type owl:Class ;
  rdfs:subClassOf :InformationBearingArtifact ;
  rdfs:label "Material Copy of a List"@en ;
  rdfs:comment "Material Copy of a List is an Information Bearing Artifact that consists of one or more Information Bearing Artifacts that carry Information Content Entities and are the subjects of some Sequence Position Ordinality."@en .

cco:ont00001002 rdf:type owl:Class ;
  rdfs:subClassOf :InformationBearingArtifact ;
  rdfs:label "Material Copy of a Message"@en ;
  rdfs:comment "Material Copy of a Message is an Information Bearing Artifact that is designed to carry some specific Information Content Entity that is relatively brief and to be transmitted from a sender to a recipient."@en .

cco:ont00000899 rdf:type owl:Class ;
  rdfs:label "Material Copy of a MSI Plessey Barcode"@en ;
  rdfs:comment "Material Copy of a MSI Plessey Barcode is a Material Copy of a One-Dimensional Barcode that consists of an indefinite number of numerical characters and is used for inventory control and marking storage containers and shelves in warehouse environments."@en .

cco:ont00001046 rdf:type owl:Class ;
  rdfs:subClassOf :MaterialCopyofaMessage ;
  rdfs:label "Material Copy of a Notification Message"@en ;
  rdfs:comment "Material Copy of a Notification Message is a Material Copy of a Message that is designed to carry an Information Content Entity that describes a scenario that has been determined to merit attention by the recipient."@en .

cco:ont00000258 rdf:type owl:Class ;
  rdfs:subClassOf :MaterialCopyofaBarcode ;
  rdfs:label "Material Copy of a One-Dimensional Barcode"@en ;
  rdfs:comment "Material Copy of a One-Dimensional Barcode is a Material Copy of a Barcode that is designed to carry parallel lines of varying widths and spacing that concretize some Directive Information Content Entity."@en .

cco:ont00001245 rdf:type owl:Class ;
  rdfs:label "Material Copy of a PDF417 Code"@en ;
  rdfs:comment "Material Copy of a PDF417 Code is a Material Copy of a Two-Dimensional Barcode that is used in applications that require the storage of huge amounts of data."@en .

cco:ont00000559 rdf:type owl:Class ;
  rdfs:label "Material Copy of a QR Code"@en ;
  rdfs:comment "Material Copy of a QR Code is a Material Copy of a Two-Dimensional Barcode that consists of numeric, alphanumeric, binary, or kanji information and is used primarily for tracking and marketing."@en .

cco:ont00000624 rdf:type owl:Class ;
  rdfs:subClassOf :MaterialCopyofaDocument ;
  rdfs:label "Material Copy of a Report"@en ;
  rdfs:comment "Material Copy of a Report is a Material Copy of a Document that is designed to carry some specific Information Content Entity that conveys an account of some event, situation, or the result of some observation or inquiry."@en .

cco:ont00000382 rdf:type owl:Class ;
  rdfs:subClassOf :MaterialCopyofaDocument ;
  rdfs:label "Material Copy of a Spreadsheet"@en ;
  rdfs:comment "Material Copy of a Spreadsheet is a Material Copy of a Document that is designed to carry some Information Content Entity in an interactive, tabular form."@en .

cco:ont00000703 rdf:type owl:Class ;
  rdfs:label "Material Copy of a System Clock"@en ;
  rdfs:comment "A Material Copy of a Timekeeping Instrument that is part of a computing device or embedded system and is designed to issue a steady high-frequency signal to synchronize internal components."@en .

cco:ont00000159 rdf:type owl:Class ;
  rdfs:subClassOf :InformationBearingArtifact ;
  rdfs:label "Material Copy of a Timekeeping Instrument"@en ;
  rdfs:comment "Material Copy of a Timekeeping Instrument is an Information Bearing Artifact that is designed to carry some specific Information Content Entity that is about some temporal region."@en .

cco:ont00000069 rdf:type owl:Class ;
  rdfs:subClassOf :MaterialCopyofaDocument ;
  rdfs:label "Material Copy of a Transcript"@en ;
  rdfs:comment "Material Copy of a Transcript is a Material Copy of a Document that is designed to carry some specific Information Content Entity that was originally recorded in a different medium."@en .

cco:ont00000241 rdf:type owl:Class ;
  rdfs:label "Material Copy of a Two-Dimensional Barcode"@en ;
  rdfs:comment "A Material Copy of a Barcode that is designed to bear modules (cells) arranged in a two-dimensional pattern that concretize some Directive Information Content Entity."@en .

cco:ont00000326 rdf:type owl:Class ;
  rdfs:label "Material Copy of a UPC Barcode"@en ;
  rdfs:comment "Material Copy of a UPC Barcode is a Material Copy of a One-Dimensional Barcode that consists of 6 or 12 numerical digits and is used to scan consumer goods."@en .

cco:ont00000931 rdf:type owl:Class ;
  rdfs:subClassOf :MaterialCopyofaUPCBarcode ;
  rdfs:label "Material Copy of a UPC-A Barcode"@en ;
  rdfs:comment "Material Copy of a UPC-A Barcode is a Material Copy of a UPC Barcode that consists of 12 numerical digits."@en .

cco:ont00001209 rdf:type owl:Class ;
  rdfs:subClassOf :MaterialCopyofaUPCBarcode ;
  rdfs:label "Material Copy of a UPC-E Barcode"@en ;
  rdfs:comment "Material Copy of a UPC-E Barcode is a Material Copy of a UPC Barcode that consists of 6 numerical digits."@en .

cco:ont00000874 rdf:type owl:Class ;
  rdfs:subClassOf :InformationBearingArtifact ;
  rdfs:label "Material Copy of a Video"@en ;
  rdfs:comment "Material Copy of a Video is an Information Bearing Artifact that is designed to carry some specific Information Content Entity in the form of a sequence of representations that are presented sufficiently rapidly to create the appearance of motion and continuity."@en .

cco:ont00000471 rdf:type owl:Class ;
  rdfs:subClassOf :MaterialCopyofaNotificationMessage ;
  rdfs:label "Material Copy of a Warning Message"@en ;
  rdfs:comment "Material Copy of a Warning Message is a Material Copy of a Notification Message that is designed to carry an Information Content Entity that describes a possible or impending threat."@en .

cco:ont00000702 rdf:type owl:Class ;
  rdfs:subClassOf :InformationBearingArtifact ;
  rdfs:label "Material Copy of an Image"@en ;
  rdfs:comment "Material Copy of an Image is an Information Bearing Artifact that is designed to carry an Information Content Entity that represents some entity owing to a visual isomorphism between the carrying artifact and the entity."@en .

cco:ont00001381 rdf:type owl:Class ;
  rdfs:subClassOf :MaterialArtifact ;
  rdfs:label "Medical Artifact"@en ;
  rdfs:comment "Medical Artifact is a Material Artifact that is designed for diagnosing, treating, or preventing disease, disability, or death."@en .

cco:ont00001217 rdf:type owl:Class ;
  rdfs:subClassOf :MountedGun ;
  rdfs:label "Medium Machine Gun"@en ;
  rdfs:comment "Medium Machine Gun is a Mounted Gun that is designed to fire full-power rifle Cartridges (less than .50 caliber or 12.7mm) in quick succession from an ammunition belt, and which typically weighs 22-30 lbs."@en .

cco:ont00000304 rdf:type owl:Class ;
  rdfs:subClassOf :ImagingInstrument ;
  rdfs:label "Microscope"@en ;
  rdfs:comment "Microscope is an Imaging Instrument that is designed to enable users to see Objects that are otherwise too small to be seen by the naked eye by producing a significantly enlarged image of the Object."@en .

cco:ont00000682 rdf:type owl:Class ;
  rdfs:subClassOf :OpticalInstrument ;
  rdfs:label "Mirror"@en ;
  rdfs:comment "Mirror is an Optical Instrument that is designed to reflect light that has a wavelength within a given range and is incident on its relflecting surface such that the reflected light maintains most of the characteristics of the original light."@en .

cco:ont00000658 rdf:type owl:Class ;
  rdfs:subClassOf :ProjectileLauncher ;
  rdfs:label "Missile Launcher"@en ;
  rdfs:comment "Missile Launcher is a Projectile Launcher that is designed to launch one or more Precision-Guided Missiles."@en .

cco:ont00000057 rdf:type owl:Class ;
  rdfs:subClassOf :Telephone ;
  rdfs:label "Mobile Telephone"@en ;
  rdfs:comment "Mobile Telephone is a Telephone that is connected to a Telephone Network by radio waves."@en .

cco:ont00000340 rdf:type owl:Class ;
  rdfs:subClassOf :Cannon ;
  rdfs:label "Mortar"@en ;
  rdfs:comment "Mortar is a Cannon that is designed to fire projectiles at relatively low velocities over relatively short ranges."@en .

cco:ont00001061 rdf:type owl:Class ;
  rdfs:label "Motorcycle"@en ;
  rdfs:comment "A Ground Motor Vehicle that is designed primarily to transport one or two passengers on two wheels; some variants include a sidecar or a third wheel."@en .

cco:ont00000848 rdf:type owl:Class ;
  rdfs:subClassOf :Firearm ;
  rdfs:label "Mounted Gun"@en ;
  rdfs:comment "Mounted Gun is a Firearm that is designed to be fired while mounted."@en .

cco:ont00001187 rdf:type owl:Class ;
  rdfs:subClassOf :MaterialArtifact ;
  rdfs:label "Navigation System"@en ;
  rdfs:comment "Navigation System is a Material Artifact that is designed to enable an Agent or Artifact to determine the position or direction of some object, usually for the purpose of monitoring or controlling the movement of some Vehicle from one place to another."@en .

cco:ont00001038 rdf:type owl:Class ;
  rdfs:subClassOf :SecondaryCellElectricBattery ;
  rdfs:label "Nickel Cadmium Electric Battery"@en ;
  rdfs:comment "Nickel Cadmium Electric Battery is a Secondary Cell Electric Battery that has a cadmium anode and nickel oxide hydroxide cathode."@en .

cco:ont00000930 rdf:type owl:Class ;
  rdfs:subClassOf :SecondaryCellElectricBattery ;
  rdfs:label "Nickel-metal Hydride Electric Battery"@en ;
  rdfs:comment "Nickel-metal Hydride Electric Battery is a Secondary Cell Electric Battery that has a metal-hydride anode and nickel oxide hydroxide cathode."@en .

cco:ont00000252 rdf:type owl:Class ;
  rdfs:subClassOf :FluidControlArtifact ,
        [ rdf:type owl:Restriction ;
      owl:onProperty :bearer_of ;
      owl:someValuesFrom cco:ont00000679
    ] ;
  rdfs:label "Nozzle"@en ;
  rdfs:comment "Nozzle is a Fluid Control Artifact that is designed to control the speed, direction, rate, shape, or pressure of the flow of fluid exiting it."@en .

cco:ont00000694 rdf:type owl:Class ;
  rdfs:subClassOf :FluidControlArtifact ;
  rdfs:label "Nozzle Mouth"@en ;
  rdfs:comment "Nozzle Mouth is a Fluid Control Artifact that consists of the portion of a Nozzle at the end that is designed to be where the flow of fluid exits the Nozzle."@en .

cco:ont00000625 rdf:type owl:Class ;
  rdfs:subClassOf :FluidControlArtifact ;
  rdfs:label "Nozzle Throat"@en ;
  rdfs:comment "Nozzle Throat is a Fluid Control Artifact that consists of the narrowest portion of a Nozzle that is designed to converge the flow of fluid in order to increase the Velocity of the flow."@en .

cco:ont00000030 rdf:type owl:Class ;
  rdfs:subClassOf :PowerSource ;
  rdfs:label "Nuclear Reactor"@en ;
  rdfs:comment "Nuclear Reactor is a Power Source that is designed to initiate and control a self-sustained nuclear chain reaction to produce power in the form of heat, which can be transferred to a working fluid for further conversion to mechanical or electrical energy."@en .

cco:ont00000277 rdf:type owl:Class ;
  rdfs:subClassOf :Weapon ;
  rdfs:label "Nuclear Weapon"@en ;
  rdfs:comment "Nuclear Weapon is a Weapon that is designed to inflict harm, damage, or incapacity by means of a destructive nuclear reaction, either through fission or through a combination of fission and fusion."@en .

cco:ont00000205 rdf:type owl:Class ;
  rdfs:label "Object Track"@en ;
  rdfs:comment "Object Track is an One-Dimensional Spatial Region that consists of the idealized line along which an Object has traversed during some motion."@en .

cco:ont00000170 rdf:type owl:Class ;
  rdfs:label "Object Track Point"@en ;
  rdfs:comment "Object Track Point is a Zero-Dimensional Spatial Region that is an idealized point where an Object is or was located during some motion."@en .

cco:ont00000943 rdf:type owl:Class ;
  rdfs:subClassOf :ArtificialEye ;
  rdfs:label "Ocular Prosthesis"@en ;
  rdfs:comment "Ocular Prosthesis is an Artificial Eye that is designed to replace a missing eye, but which does not function as an eye."@en .

cco:ont00000869 rdf:type owl:Class ;
  rdfs:subClassOf :Camera ;
  rdfs:label "Optical Camera"@en ;
  rdfs:comment "Optical Camera is a Camera that is designed to form and record an image generated from visible light."@en .

cco:ont00000136 rdf:type owl:Class ;
  rdfs:subClassOf :MaterialArtifact ;
  rdfs:label "Optical Instrument"@en ;
  rdfs:comment "Optical Instrument is a Material Artifact that is designed to process light waves."@en .

cco:ont00001207 rdf:type owl:Class ;
  rdfs:subClassOf :OpticalInstrument ;
  rdfs:label "Optical Lens"@en ;
  rdfs:comment "Optical Lens is an Optical Instrument that is designed to focus or disperse a beam of light entering the lens by means of refraction."@en .

cco:ont00000075 rdf:type owl:Class ;
  rdfs:subClassOf :Microscope ;
  rdfs:label "Optical Microscope"@en ;
  rdfs:comment "Optical Microscope is a Microscope that is designed to use visible light and a system of Optical Lenses to produce a significantly enlarged image of the Object."@en .

cco:ont00001009 rdf:type owl:Class ;
  rdfs:subClassOf :Telescope ;
  rdfs:label "Optical Telescope"@en ;
  rdfs:comment "Optical Telescope is a Telescope that is designed to aid in the observation of spatially distant Objects by means of collecting and focusing visible light to form an enhanced image of the Object."@en .

cco:ont00000724 rdf:type owl:Class ;
  rdfs:subClassOf :RadioAntenna ;
  rdfs:label "Parabolic Antenna"@en ;
  rdfs:comment "Parabolic Antenna is a Radio Antenna that uses a parabolic reflector to direct or receive radio waves and has a very high gain."@en .

cco:ont00000929 rdf:type owl:Class ;
  rdfs:subClassOf :Role ;
  rdfs:label "Part Role"@en ;
  rdfs:comment "Part Role is a Role that inheres in an entity in virtue of it being part of some other entity without being subject to further subdivision or disassembly without destruction of its designated use."@en .

cco:ont00000919 rdf:type owl:Class ;
  rdfs:subClassOf :QualitySpecification ;
  rdfs:label "Parts List"@en ;
  rdfs:comment "Parts List is a Quality Specification that prescribes the Amount of some type of Artifact that are part of or located on another Artifact."@en .

cco:ont00001007 rdf:type owl:Class ;
  rdfs:subClassOf :TrainCar ;
  rdfs:label "Passenger Train Car"@en ;
  rdfs:comment "Passenger Train Car is a Train Car that is designed to transport passengers."@en .

cco:ont00001300 rdf:type owl:Class ;
  rdfs:subClassOf :RadioAntenna ;
  rdfs:label "Patch Antenna"@en ;
  rdfs:comment "Patch Antenna is a Radio Antenna that consists of a flat rectangular sheet (or patch) of metal mounted over a larger sheet of metal called a ground plane which is typically contained inside a plastic radome for protection and is small enough that it can be mounted on a flat surface."@en .

cco:ont00001082 rdf:type owl:Class ;
  rdfs:subClassOf :RadioReceiver ;
  rdfs:label "Patch Receiver"@en ;
  rdfs:comment "Patch Receiver is a Radio Receiver that uses a Patch Antenna to intercept radio signals."@en .

cco:ont00000556 rdf:type owl:Class ;
  rdfs:subClassOf :MaterialEntity ;
  rdfs:label "Payload"@en ;
  rdfs:comment "Payload is a Material Entity that is transported by a Vehicle during an Act of Location Change for the purpose of being delivered to or performing one or more functions at a predefined location."@en .

cco:ont00001071 rdf:type owl:Class ;
  rdfs:subClassOf :ArtifactFunction ;
  rdfs:label "Payload Capacity"@en ;
  rdfs:comment "Payload Capacity is an Artifact Function that inheres in a Vehicle that is designed to transport Payload, and which is typically characterized by the maximum Weight, Mass, or Volume of Payload that the Vehicle can transport."@en .

cco:ont00001216 rdf:type owl:Class ;
  rdfs:subClassOf :OpticalInstrument ,
        [ rdf:type owl:Restriction ;
      owl:onProperty :bearer_of ;
      owl:someValuesFrom cco:ont00001368
    ] ;
  rdfs:label "Periscope"@en ;
  rdfs:comment "Periscope is an Optical Instrument that is designed to enable observation of an object that is located over, around, or through another object, obstacle, or condition that prevents direct line-of-sight observation from the observer's current position."@en .

cco:ont00001221 rdf:type owl:Class ;
  rdfs:subClassOf :Engine ;
  rdfs:label "Physically Powered Engine"@en ;
  rdfs:comment "Physically Powered Engine is an Engine that is designed to convert potential or kinetic energy into mechanical energy."@en .

cco:ont00000364 rdf:type owl:Class ;
  rdfs:subClassOf :PhysicallyPoweredEngine ;
  rdfs:label "Pneumatic Motor"@en ;
  rdfs:comment "Pneumatic Motor is a Physically Powered Engine that converts potential energy stored in a portion of compressed air into mechanical energy."@en .

cco:ont00000516 rdf:type owl:Class ;
  rdfs:subClassOf :PowerSource ;
  rdfs:label "Pneumatic Power Source"@en ;
  rdfs:comment "Pneumatic Power Source is a Power Source that is designed to generate, control, or transmit power by means of compressed air or compressed inert gases."@en .

cco:ont00000721 rdf:type owl:Class ;
  rdfs:subClassOf :Prism ;
  rdfs:label "Polarizing Prism"@en ;
  rdfs:comment "Polarizing Prism is a Prism designed to split a beam of light entering the Prism into components of varying polarization."@en .

cco:ont00001150 rdf:type owl:Class ;
  rdfs:subClassOf :Weapon ;
  rdfs:label "Portion of Ammunition"@en ;
  rdfs:comment "Portion of Ammunition is a Weapon that is designed to inflict harm, damage, or incapacity by being projected toward its target at a significant Velocity."@en .

cco:ont00000475 rdf:type owl:Class ;
  rdfs:subClassOf :FinancialInstrument ;
  rdfs:label "Portion of Cash"@en ;
  rdfs:comment "Portion of Cash is a Financial Instrument that is designed to be a ready medium of exchange."@en .

cco:ont00000091 rdf:type owl:Class ;
  rdfs:subClassOf :PortionofMaterial ;
  rdfs:label "Portion of Coolant"@en ;
  rdfs:comment "Portion of Coolant is a Portion of Material that is designed to be used in a thermal control system to reduce or maintain the temperature of an object to or at a specified level."@en .

cco:ont00000255 rdf:type owl:Class ;
  rdfs:subClassOf :PortionofMaterial ;
  rdfs:label "Portion of Cryogenic Material"@en ;
  rdfs:comment "Portion of Cryogenic Material is a Portion of Material that has been reduced to a very low temperature (below -180 degrees Celcius)."@en .

cco:ont00000307 rdf:type owl:Class ;
  rdfs:subClassOf :PortionofProcessedMaterial ;
  rdfs:label "Portion of Food"@en ;
  rdfs:comment "Portion of Food is a Portion of Processed Material that is designed to be consumed and ingested for nutrition or taste."@en .

cco:ont00000838 rdf:type owl:Class ;
  rdfs:subClassOf :PortionofMaterial ;
  rdfs:label "Portion of Fuel"@en ;
  rdfs:comment "Portion of Fuel is a Portion of Material that is designed to release thermal energy when reacted with other substances."@en .

cco:ont00000376 rdf:type owl:Class ;
  rdfs:subClassOf :PortionofMaterial ;
  rdfs:label "Portion of Gallium Arsenide"@en ;
  rdfs:comment "Portion of Gallium Arsenide is a Portion of Material that is composed of a compound of the elements gallium and arsenic."@en .

cco:ont00001020 rdf:type owl:Class ;
  rdfs:subClassOf :PortionofFuel ;
  rdfs:label "Portion of Gaseous Fuel"@en ;
  rdfs:comment "Portion of Gaseous Fuel is a Portion of Fuel that is stored in a gaseous state."@en .

cco:ont00000637 rdf:type owl:Class ;
  rdfs:subClassOf :PortionofPropellant ;
  rdfs:label "Portion of Gaseous Propellant"@en ;
  rdfs:comment "Portion of Gaseous Propellant is a Portion of Propellant that is stored in a gaseous state."@en .

cco:ont00001172 rdf:type owl:Class ;
  rdfs:subClassOf :PortionofPropellant ;
  rdfs:label "Portion of Gelatinous Propellant"@en ;
  rdfs:comment "Portion of Gelatinous Propellant is a Portion of Propellant that is stored in a gelatinous state."@en .

cco:ont00001341 rdf:type owl:Class ;
  rdfs:subClassOf :fiatobjectpart ;
  rdfs:label "Portion of Geosphere"@en ;
  rdfs:comment "Portion of Geosphere is a fiat object part that is composed of one or more portions of the atmosphere, cryosphere, hydrosphere, or lithosphere."@en .

cco:ont00001135 rdf:type owl:Class ;
  rdfs:subClassOf :PortionofFuel ;
  rdfs:label "Portion of Liquid Fuel"@en ;
  rdfs:comment "Portion of Liquid Fuel is a Portion of Fuel that is stored in a liquid state."@en .

cco:ont00000316 rdf:type owl:Class ;
  rdfs:subClassOf :PortionofCryogenicMaterial ;
  rdfs:label "Portion of Liquid Helium"@en ;
  rdfs:comment "Portion of Liquid Helium is a Portion of Cryogenic Material that is composed (almost) entirely of liquid helium."@en .

cco:ont00000128 rdf:type owl:Class ;
  rdfs:subClassOf :PortionofCryogenicMaterial ;
  rdfs:label "Portion of Liquid Hydrogen"@en ;
  rdfs:comment "Portion of Liquid Hydrogen is a Portion of Cryogenic Material that is composed (almost) entirely of liquid hydrogen."@en .

cco:ont00000816 rdf:type owl:Class ;
  rdfs:subClassOf :PortionofCryogenicMaterial ;
  rdfs:label "Portion of Liquid Nitrogen"@en ;
  rdfs:comment "Portion of Liquid Nitrogen is a Portion of Cryogenic Material that is composed (almost) entirely of liquid nitrogen."@en .

cco:ont00000101 rdf:type owl:Class ;
  rdfs:subClassOf :PortionofCryogenicMaterial ;
  rdfs:label "Portion of Liquid Oxygen"@en ;
  rdfs:comment "Portion of Liquid Oxygen is a Portion of Cryogenic Material that is composed (almost) entirely of liquid oxygen."@en .

cco:ont00000962 rdf:type owl:Class ;
  rdfs:subClassOf :PortionofPropellant ;
  rdfs:label "Portion of Liquid Propellant"@en ;
  rdfs:comment "Portion of Liquid Propellant is a Portion of Propellant that is stored in a liquid state."@en .

cco:ont00000457 rdf:type owl:Class ;
  rdfs:subClassOf :PortionofProcessedMaterial ;
  rdfs:label "Portion of Material"@en ;
  rdfs:comment "Portion of Material is a Portion of Processed Material that was produced to be used as the input for another Act of Artifact Processing."@en .

cco:ont00000813 rdf:type owl:Class ;
  rdfs:subClassOf :PortionofMaterial ;
  rdfs:label "Portion of Nuclear Fuel"@en ;
  rdfs:comment "Portion of Nuclear Fuel is a Portion of Material that is designed to be used in a nuclear fission process to produce energy."@en .

cco:ont00000897 rdf:type owl:Class ;
  rdfs:subClassOf :PortionofMaterial ;
  rdfs:label "Portion of Oxidizer"@en ;
  rdfs:comment "Portion of Oxidizer is a Portion of Material that is disposed to steal electrons from other substances (i.e. to oxidize other substances) as a participant in a reduction-oxidation process."@en .

cco:ont00001151 rdf:type owl:Class ;
  rdfs:subClassOf :InformationMediumArtifact ;
  rdfs:label "Portion of Paper"@en ;
  rdfs:comment "Portion of Paper is an Information Medium Artifact that is designed to bear some Information Content Entity by means of pressing together moist fibres of cellulose pulp derived from wood, rags, or grasses, and drying them into flexible sheets."@en .

cco:ont00001084 rdf:type owl:Class ;
  rdfs:subClassOf :MaterialArtifact ;
  rdfs:label "Portion of Processed Material"@en ;
  rdfs:comment "Portion of Processed Material is a Material Artifact that is the output of an Act of Artifact Processing."@en .

cco:ont00000593 rdf:type owl:Class ;
  rdfs:subClassOf :PortionofMaterial ;
  rdfs:label "Portion of Propellant"@en ;
  rdfs:comment "Portion of Propellant is a Portion of Material that is designed to be used as an input in a Propulsion Process to produce Thrust."@en .

cco:ont00000039 rdf:type owl:Class ;
  rdfs:subClassOf :PortionofFuel ;
  rdfs:label "Portion of Solid Fuel"@en ;
  rdfs:comment "Portion of Solid Fuel is a Portion of Fuel that is stored in a solid state."@en .

cco:ont00000043 rdf:type owl:Class ;
  rdfs:subClassOf :PortionofPropellant ;
  rdfs:label "Portion of Solid Propellant"@en ;
  rdfs:comment "Portion of Solid Propellant is a Portion of Propellant that is stored in a solid state."@en .

cco:ont00000980 rdf:type owl:Class ;
  rdfs:subClassOf :PortionofProcessedMaterial ;
  rdfs:label "Portion of Waste Material"@en ;
  rdfs:comment "Portion of Waste Material is a Portion of Processed Material that serves no further use in terms of the initial user's own purposes of production, transformation, or consumption such that the Agent wants to dispose of it."@en .

cco:ont00000577 rdf:type owl:Class ;
  rdfs:subClassOf :MaterialArtifact ;
  rdfs:label "Power Rectifier"@en ;
  rdfs:comment "Power Rectifier is a Material Artifact that is designed to convert alternating current (AC) to direct current (DC)."@en .

cco:ont00000288 rdf:type owl:Class ;
  rdfs:subClassOf :MaterialArtifact ,
        [ rdf:type owl:Restriction ;
      owl:onProperty :bearer_of ;
      owl:someValuesFrom cco:ont00000994
    ] ;
  rdfs:label "Power Source"@en ;
  rdfs:comment "Power Source is a Material Artifact that is designed to supply power to some other Artifact."@en .

cco:ont00000806 rdf:type owl:Class ;
  rdfs:subClassOf :Tool ;
  rdfs:label "Power Tool"@en ;
  rdfs:comment "Power Tool is a Tool that is designed to be actuated by a Power Source and mechanism other than or in addition to manual labor."@en .

cco:ont00000130 rdf:type owl:Class ;
  rdfs:subClassOf :MaterialArtifact ,
        [ rdf:type owl:Restriction ;
      owl:onProperty :bearer_of ;
      owl:someValuesFrom cco:ont00000098
    ] ;
  rdfs:label "Power Transformer"@en ;
  rdfs:comment "Power Transformer is a Material Artifact that is designed to transfer electrical energy between two or more circuits through electromagnetic induction."@en .

cco:ont00000372 rdf:type owl:Class ;
  rdfs:subClassOf :MaterialArtifact ;
  rdfs:label "Power Transformer Rectifier Unit"@en ;
  rdfs:comment "Power Transformer Rectifier Unit is a Material Artifact that is designed to perform the functions of both a Rectifier and a Transformer."@en .

cco:ont00000663 rdf:type owl:Class ;
  rdfs:subClassOf :MaterialArtifact ;
  rdfs:label "Power Transmission Artifact"@en ;
  rdfs:comment "Power Transmission Artifact is a Material Artifact that is designed to transfer and regulate Power flow from a Power Source to an application point."@en .

cco:ont00001124 rdf:type owl:Class ;
  rdfs:subClassOf :PortionofAmmunition ;
  rdfs:label "Precision-Guided Missile"@en ;
  rdfs:comment "Precision-Guided Missile is a Portion of Ammunition that is designed to be a self-propelled and precision-guided projectile that delivers some payload (explosive or other) over relatively long distances."@en .

cco:ont00000093 rdf:type owl:Class ;
  rdfs:subClassOf :Stock ;
  rdfs:label "Preferred Stock"@en ;
  rdfs:comment "Preferred Stock is a Stock that entitles its holder to receive a certain level of dividend payments before any dividends can be issued to other holders."@en .

cco:ont00001050 rdf:type owl:Class ;
  rdfs:subClassOf :ElectricBattery ;
  rdfs:label "Primary Cell Electric Battery"@en ;
  rdfs:comment "Primary Cell Electric Battery is an Electric Battery that is designed for one-time use and not to be recharged."@en .

cco:ont00000804 rdf:type owl:Class ;
  rdfs:subClassOf :OpticalInstrument ;
  rdfs:label "Prism"@en ;
  rdfs:comment "Prism is an Optical Instrument that is designed to refract light and which consists of a transparent material with flat polished surfaces where at least two of these surfaces have an angle between them."@en .

cco:ont00001051 rdf:type owl:Class ;
  rdfs:subClassOf :Weapon ;
  rdfs:label "Projectile Launcher"@en ;
  rdfs:comment "Projectile Launcher is a Weapon that is designed to inflict damage or harm by means of launching a high-velocity projectile at a target."@en .

cco:ont00000238 rdf:type owl:Class ;
  rdfs:subClassOf :MaterialArtifact ,
        [ rdf:type owl:Restriction ;
      owl:onProperty :bearer_of ;
      owl:someValuesFrom cco:ont00001155
    ] ;
  rdfs:label "Propeller"@en ;
  rdfs:comment "Propeller is a Material Artifact that is designed to convert rotary motion from an Engine or other mechanical Power Source into propulsive Force."@en .

cco:ont00001117 rdf:type owl:Class ;
  rdfs:label "Propelling Nozzle"@en ;
  rdfs:comment "A Nozzle that is designed to accelerate and shape engine exhaust to produce thrust as part of a reaction (jet) engine, typically by choking flow at the throat and expanding the exhaust to form a high-speed jet."@en .

cco:ont00000012 rdf:type owl:Class ;
  rdfs:subClassOf :ControlSystem ,
        [ rdf:type owl:Restriction ;
      owl:onProperty :bearer_of ;
      owl:someValuesFrom cco:ont00000679
    ] ;
  rdfs:label "Propulsion Control System"@en ;
  rdfs:comment "Propulsion Control System is a Control System that consists of control devices, displays, indicators, or modules designed to control a Propulsion System."@en .

cco:ont00000096 rdf:type owl:Class ;
  rdfs:subClassOf :MaterialArtifact ;
  rdfs:label "Propulsion System"@en ;
  rdfs:comment "Propulsion System is a Material Artifact that is designed to facilitate the movement of material entities from one location to another and which consists of a source of mechanical power and a means of converting this power into propulsive force to generate the movement."@en .

cco:ont00000715 rdf:type owl:Class ;
  rdfs:subClassOf :MedicalArtifact ;
  rdfs:label "Prosthesis"@en ;
  rdfs:comment "Prosthesis is a Medical Artifact that is designed to replace a missing body part."@en .

cco:ont00000341 rdf:type owl:Class ;
  rdfs:subClassOf :Prosthesis ;
  rdfs:label "Prosthetic Arm"@en ;
  rdfs:comment "Prosthetic Arm is a Prosthesis that is designed to replace a missing arm."@en .

cco:ont00000673 rdf:type owl:Class ;
  rdfs:subClassOf :Prosthesis ;
  rdfs:label "Prosthetic Foot"@en ;
  rdfs:comment "Prosthetic Foot is a Prosthesis that is designed to replace a missing foot."@en .

cco:ont00000417 rdf:type owl:Class ;
  rdfs:subClassOf :Prosthesis ;
  rdfs:label "Prosthetic Hand"@en ;
  rdfs:comment "Prosthetic Hand is a Prosthesis that is designed to replace a missing hand."@en .

cco:ont00000299 rdf:type owl:Class ;
  rdfs:subClassOf :Prosthesis ;
  rdfs:label "Prosthetic Leg"@en ;
  rdfs:comment "Prosthetic Leg is a Prosthesis that is designed to replace a missing leg."@en .

cco:ont00001265 rdf:type owl:Class ;
  rdfs:label "Public Address System"@en ;
  rdfs:comment "A Communication System that is designed to amplify and distribute audio so a speaker can be heard by multiple listeners within a shared space."@en .

cco:ont00000522 rdf:type owl:Class ;
  rdfs:label "Pulsejet Engine"@en ;
  rdfs:comment "Pulsejet Engine is an Air-Breathing Jet Engine that is capable of operating statically and uses intermittent (pulsing) Combustion of the fuel-oxidizer mixture before expelling the exhaust out through the rear Propelling Nozzle to generate Thrust."@en .

cco:ont00000116 rdf:type owl:Class ;
  rdfs:subClassOf :FluidControlArtifact ,
        [ rdf:type owl:Restriction ;
      owl:onProperty :bearer_of ;
      owl:someValuesFrom cco:ont00001155
    ] ;
  rdfs:label "Pump"@en ;
  rdfs:comment "Pump is a Fluid Control Artifact that is designed to impart motion to a portion of fluid to transport it within a system through the use of mechanical action."@en .

cco:ont00000575 rdf:type owl:Class ;
  rdfs:subClassOf :DirectiveInformationContentEntity ;
  rdfs:label "Quality Specification"@en ;
  rdfs:comment "Quality Specification is a Directive Information Content Entity that prescribes some Quality."@en .

cco:ont00001192 rdf:type owl:Class ;
  rdfs:subClassOf :BidirectionalTransducer ,
        [ rdf:type owl:Restriction ;
      owl:onProperty :bearer_of ;
      owl:someValuesFrom cco:ont00000994
    ] ;
  rdfs:label "Radio Antenna"@en ;
  rdfs:comment "Radio Antenna is a Bidirectional Transducer that is designed to convert electric power into radio waves, and radio waves into electric power."@en .

cco:ont00000903 rdf:type owl:Class ;
  rdfs:subClassOf :CommunicationInstrument ,
        [ rdf:type owl:Restriction ;
      owl:onProperty :bearer_of ;
      owl:someValuesFrom cco:ont00000727
    ] ;
  rdfs:label "Radio Communication Instrument"@en ;
  rdfs:comment "Radio Communication Instrument is a Communication Instrument that is designed to enable communication between two or more entities via the use of radio waves."@en .

cco:ont00001145 rdf:type owl:Class ;
  rdfs:subClassOf :RadioCommunicationInstrument ;
  rdfs:label "Radio Receiver"@en ;
  rdfs:comment "Radio Receiver is a Radio Communication Instrument that is an electronic device that is designed to extract information from radio waves intercepted by a Radio Antenna by using electronic filters to separate the desired radio frequency signal from other signals, an electronic amplifier to increase the power of the signal, and demodulation to recover the desired information."@en .

cco:ont00000785 rdf:type owl:Class ;
  rdfs:subClassOf :RadioTransceiver ;
  rdfs:label "Radio Repeater"@en ;
  rdfs:comment "Radio Repeater is a Radio Transceiver that is designed to receive a radio signal, amplify it, and retransmit it (often on another frequency)."@en .

cco:ont00000215 rdf:type owl:Class ;
  rdfs:subClassOf :Telescope ;
  rdfs:label "Radio Telescope"@en ;
  rdfs:comment "Radio Telescope is a Telescope that is designed to aid in the observation of spatially distant Objects by means of collecting and focusing radio waves to form an enhanced image of the Object."@en .

cco:ont00001320 rdf:type owl:Class ;
  rdfs:subClassOf :RadioCommunicationInstrument ;
  rdfs:label "Radio Transceiver"@en ;
  rdfs:comment "Radio Transceiver is a Radio Communication Instrument that is an electronic device composed of both a Radio Transmitter and a Radio Receiver that share common circuitry or a single housing."@en .

cco:ont00000269 rdf:type owl:Class ;
  rdfs:subClassOf :RadioCommunicationInstrument ;
  rdfs:label "Radio Transmitter"@en ;
  rdfs:comment "Radio Transmitter is a Radio Communication Instrument that is an electronic device that is designed to generate a radio frequency alternating current, which can be applied to a Radio Antenna to be transmitted as radio waves."@en .

cco:ont00000325 rdf:type owl:Class ;
  rdfs:subClassOf :RadioCommunicationInstrument ;
  rdfs:label "Radio Transponder"@en ;
  rdfs:comment "Radio Transponder is a Radio Communication Instrument that is an electronic device that acts as both a Radio Transmitter and responder and is used to wirelessly receive and transmit electrical signals."@en .

cco:ont00000656 rdf:type owl:Class ;
  rdfs:subClassOf :Weapon ;
  rdfs:label "Radiological Weapon"@en ;
  rdfs:comment "Radiological Weapon is a Weapon that is designed to inflict harm, damage, or incapacity by means of releasing radioactive material."@en .

cco:ont00000796 rdf:type owl:Class ;
  rdfs:subClassOf :GroundVehicle ;
  rdfs:label "Rail Transport Vehicle"@en ;
  rdfs:comment "Rail Transport Vehicle is a Ground Vehicle that is designed to convey cargo, passengers, or equipment by Railway."@en .

cco:ont00001198 rdf:type owl:Class ;
  rdfs:label "Railcar"@en ;
  rdfs:comment "A Rail Transport Vehicle that consists of a single vehicle designed to carry passengers or cargo; it may be unpowered (hauled) or self-propelled and may couple with other railcars to form a train."@en .

cco:ont00000456 rdf:type owl:Class ;
  rdfs:subClassOf :LandTransportationArtifact ;
  rdfs:label "Railway"@en ;
  rdfs:comment "Railway is a Land Transportation Artifact that is designed to enable Trains to transport passengers and goods."@en .

cco:ont00001178 rdf:type owl:Class ;
  rdfs:subClassOf :LandTransportationArtifact ,
        [ rdf:type owl:Restriction ;
      owl:onProperty :bearer_of ;
      owl:someValuesFrom cco:ont00000650
    ] ;
  rdfs:label "Railway Crossing"@en ;
  rdfs:comment "Railway Crossing is a Land Transportation Artifact that is designed to enable Persons or Ground Vehicles to cross a Railway when traveling along a road or path that is perpendicular to and at the same elevation as the Railway at the point where they overlap."@en .

cco:ont00000428 rdf:type owl:Class ;
  rdfs:subClassOf :LandTransportationArtifact ;
  rdfs:label "Railway Junction"@en ;
  rdfs:comment "Railway Junction is a Land Transportation Artifact that is designed to enable a Train to switch between the tracks of two routes."@en .

cco:ont00000996 rdf:type owl:Class ;
  rdfs:label "Ramjet Engine"@en ;
  rdfs:comment "Ramjet Engine is an Air-Breathing Jet Engine that uses the forward motion of the Engine to compress incoming air (without the use of an axial compressor) and decelerate it to subsonic speeds before adding the fuel and constantly combusting the mixture then expelling the exhaust out through the rear Propelling Nozzle to generate Thrust."@en .

cco:ont00000048 rdf:type owl:Class ;
  rdfs:subClassOf :WireAntenna ;
  rdfs:label "Random Wire Antenna"@en ;
  rdfs:comment "Random Wire Antenna is a Wire Antenna that consists of a long wire suspended above the ground with a length that does not bear a relation to the wavelength of the radio waves used and which is typically used as a receiving antenna on the long, medium, and short wave bands."@en .

cco:ont00000056 rdf:type owl:Class ;
  rdfs:subClassOf :Engine ;
  rdfs:label "Reaction Engine"@en ;
  rdfs:comment "Reaction Engine is an Engine that provides propulsion by expelling Reaction Mass."@en .

cco:ont00001168 rdf:type owl:Class ;
  rdfs:subClassOf :MaterialEntityagainst ;
  rdfs:label "Reaction Mass"@en ;
  rdfs:comment "Reaction Mass is a Material Entity against that a Propulsion System operates in order to produce Acceleration."@en .

cco:ont00000343 rdf:type owl:Class ;
  rdfs:subClassOf :SteamEngine ;
  rdfs:label "Reciprocating Steam Engine"@en ;
  rdfs:comment "Reciprocating Steam Engine is a Steam Engine that is designed to use one or more reciprocating pistons to convert pressure into a rotating motion."@en .

cco:ont00000132 rdf:type owl:Class ;
  rdfs:subClassOf :InformationProcessingArtifact ;
  rdfs:label "Recording Device"@en ;
  rdfs:comment "Recording Device is an Information Processing Artifact that is designed to capture some information and store it in some recording format on some storage medium."@en .

cco:ont00000219 rdf:type owl:Class ;
  rdfs:subClassOf :OpticalTelescope ;
  rdfs:label "Reflecting Optical Telescope"@en ;
  rdfs:comment "Reflecting Optical Telescope is an Optical Telescope that is designed to aid in the observation of spatially distant Objects by means of collecting and focusing visible light via reflection through the use of one or more curved Mirrors to form an enhanced image of the Object."@en .

cco:ont00000988 rdf:type owl:Class ;
  rdfs:subClassOf :Prism ;
  rdfs:label "Reflective Prism"@en ;
  rdfs:comment "Reflective Prism is a Prism designed to reflect light in order to flip, invert, rotate, deviate, or displace a beam of light entering the Prism."@en .

cco:ont00000355 rdf:type owl:Class ;
  rdfs:subClassOf :OpticalTelescope ;
  rdfs:label "Refracting Optical Telescope"@en ;
  rdfs:comment "Refracting Optical Telescope is an Optical Telescope that is designed to aid in the observation of spatially distant Objects by means of collecting and focusing visible light via refraction through the use of one or more Lenses to form an enhanced image of the Object."@en .

cco:ont00000740 rdf:type owl:Class ;
  rdfs:subClassOf :Continuant ;
  rdfs:label "Resource"@en ;
  rdfs:comment "Resource is a Continuant that is owned by, in the possession of, or is otherwise controlled by an Agent such that it could be used by that Agent."@en .

cco:ont00001254 rdf:type owl:Class ;
  rdfs:label "Revolver"@en ;
  rdfs:comment "Revolver is a Hand Gun having a number of firing chambers in a revolving cylinder, where each chamber in the cylinder can be loaded with a single Cartridge."@en .

cco:ont00001230 rdf:type owl:Class ;
  rdfs:subClassOf :WireAntenna ;
  rdfs:label "Rhombic Antenna"@en ;
  rdfs:comment "Rhombic Antenna is a Wire Antenna that consists of one to three parallel wires suspended above the ground by poles or towers at each vertex in a rhombic shape with each of the four sides being the same length (typically at least one wavelength or longer)."@en .

cco:ont00000204 rdf:type owl:Class ;
  rdfs:subClassOf :LongGun ;
  rdfs:label "Rifle"@en ;
  rdfs:comment "Rifle is a Long Gun that is designed to have a rifled barrel and to fire single Bullets over long ranges with high accuracy."@en .

cco:ont00000247 rdf:type owl:Class ;
  rdfs:subClassOf :LandTransportationArtifact ,
        [ rdf:type owl:Restriction ;
      owl:onProperty :bearer_of ;
      owl:someValuesFrom cco:ont00000650
    ] ;
  rdfs:label "Road"@en ;
  rdfs:comment "Road is a Land Transportation Artifact that is designed to enable Ground Vehicles to travel from one location to another."@en .

cco:ont00001086 rdf:type owl:Class ;
  rdfs:subClassOf :LandTransportationArtifact ,
        [ rdf:type owl:Restriction ;
      owl:onProperty :bearer_of ;
      owl:someValuesFrom cco:ont00000650
    ] ;
  rdfs:label "Road Junction"@en ;
  rdfs:comment "Road Junction is a Land Transportation Artifact that is designed to enable Ground Vehicles to exit one Road and enter another."@en .

cco:ont00001185 rdf:type owl:Class ;
  rdfs:subClassOf :Vehicle ;
  rdfs:label "Rocket"@en ;
  rdfs:comment "Rocket is a Vehicle that is designed to travel through air or space and which obtains Thrust from a Rocket Engine."@en .

cco:ont00000362 rdf:type owl:Class ;
  rdfs:subClassOf :JetEngine ;
  rdfs:label "Rocket Engine"@en ;
  rdfs:comment "Rocket Engine is a Jet Engine that is designed to use only stored Rocket Propellant to form a high speed propulsive jet in order to generate Thrust."@en .

cco:ont00001173 rdf:type owl:Class ;
  rdfs:subClassOf :ProjectileLauncher ;
  rdfs:label "Rocket Launcher"@en ;
  rdfs:comment "Rocket Launcher is a Projectile Launcher that is designed to launch one or more Unguided Rockets."@en .

cco:ont00000868 rdf:type owl:Class ;
  rdfs:subClassOf :RocketLauncher ;
  rdfs:label "Rocket Pod"@en ;
  rdfs:comment "Rocket Pod is a Rocket Launcher that is designed to contain several Unguided Rockets held in individual tubes and to be used by Aircraft or Helicopters for close air support."@en .

cco:ont00000337 rdf:type owl:Class ;
  rdfs:label "Rocket-Propelled Grenade"@en ;
  rdfs:comment "An unguided, shoulder-fired rocket with an explosive warhead that is designed to be used against armored and material targets."@en .

cco:ont00001288 rdf:type owl:Class ;
  rdfs:subClassOf :PortionofAmmunition ;
  rdfs:label "Round Shot"@en ;
  rdfs:comment "Round Shot is a Portion of Ammunition that is designed to be a solid projectile without explosive charge and to be fired from a cannon."@en .

cco:ont00000352 rdf:type owl:Class ;
  rdfs:subClassOf :Spacecraft ;
  rdfs:label "Satellite Artifact"@en ;
  rdfs:comment "Satellite Artifact is a Spacecraft that is designed to Orbit a Space Object (typically Earth)."@en .

cco:ont00001121 rdf:type owl:Class ;
  rdfs:label "Scramjet Engine"@en ;
  rdfs:comment "Scramjet Engine is an Air-Breathing Jet Engine that uses the forward motion of the Engine to compress incoming air at supersonic speeds before adding the fuel and constantly combusting the mixture then expelling the exhaust out through the rear Propelling Nozzle to generate Thrust."@en .

cco:ont00001105 rdf:type owl:Class ;
  rdfs:subClassOf :ElectricBattery ;
  rdfs:label "Secondary Cell Electric Battery"@en ;
  rdfs:comment "Secondary Cell Electric Battery is an Electric Battery that is designed to be recharged."@en .

cco:ont00000711 rdf:type owl:Class ;
  rdfs:subClassOf :HandGun ;
  rdfs:label "Semi-automatic Pistol"@en ;
  rdfs:comment "Semi-automatic Pistol is a Hand Gun that has a single fixed firing chamber machined into the rear of the barrel and an ammunition magazine capable of holding multiple Cartridges such that the Hand Gun is designed to automatically reload each time it is fired and to fire a Bullet with each successive pull of the trigger until the stored ammunition is depleted."@en .

cco:ont00000569 rdf:type owl:Class ;
  rdfs:subClassOf :Transducer ;
  rdfs:label "Sensor"@en ;
  rdfs:comment "Sensor is a Transducer that is designed to convert incoming energy into a output signal which reliably corresponds to changes in that energy."@en .

cco:ont00000021 rdf:type owl:Class ;
  rdfs:subClassOf :MaterialArtifact ;
  rdfs:label "Sensor Platform"@en ;
  rdfs:comment "Sensor Platform is a Material Artifact that is designed to support, and in some cases transport, a Sensor during its deployment and functioning."@en .

cco:ont00000249 rdf:type owl:Class ;
  rdfs:subClassOf :MaterialArtifact ;
  rdfs:label "Shaft"@en ;
  rdfs:comment "Shaft is a Material Artifact that is designed to rotate and transmit Torque, Power, or Rotational Motion from one machine element to another."@en .

cco:ont00000216 rdf:type owl:Class ;
  rdfs:subClassOf :PortionofAmmunition ;
  rdfs:label "Shell"@en ;
  rdfs:comment "Shell is a Portion of Ammunition that is designed to be a non-self-propelled projectile and to carry a payload (explosive or other) over a relatively short distance."@en .

cco:ont00000015 rdf:type owl:Class ;
  rdfs:subClassOf :LongGun ;
  rdfs:label "Shotgun"@en ;
  rdfs:comment "Shotgun is a Long Gun that fires packets of shot, a single slug, a sabot, or a specialty round (such as tear gas, bolo shell, or a breaching round) over shorter ranges than that of Rifles and with less accuracy."@en .

cco:ont00000298 rdf:type owl:Class ;
  rdfs:subClassOf :RocketLauncher ;
  rdfs:label "Shoulder-Fired Rocket Launcher"@en ;
  rdfs:comment "Shoulder-Fired Rocket Launcher is a Rocket Launcher that is designed to be small enough to be carried by a single person and fired while supported on the person's shoulder."@en .

cco:ont00000434 rdf:type owl:Class ;
  rdfs:label "Simple Optical Lens"@en ;
  rdfs:comment "Simple Optical Lens is an Optical Lens consisting of a single piece of transparent material."@en .

cco:ont00000942 rdf:type owl:Class ;
  rdfs:subClassOf :Rifle ;
  rdfs:label "Sniper Rifle"@en ;
  rdfs:comment "Sniper Rifle is a Rifle that is designed to be highly accurate for long-range precision tactical shooting."@en .

cco:ont00000843 rdf:type owl:Class ;
  rdfs:subClassOf :ElectricalPowerSource ;
  rdfs:label "Solar Panel"@en ;
  rdfs:comment "Solar Panel is an Electrical Power Source that consists in part of one or more photovoltaic (i.e. solar) cells that convert light energy (photons) directly into electricity by means of the photovoltaic effect."@en .

cco:ont00001222 rdf:type owl:Class ;
  rdfs:subClassOf :ElectricalPowerSource ;
  rdfs:label "Solar Panel System"@en ;
  rdfs:comment "Solar Panel System is an Electrical Power Source that consists in part of one or more Solar Panels, a power inverter, electrical wiring between the components, a mounting and support structure, and may also include a battery and/or a solar tracking system and is the bearer of functions realized in processes of deriving, transferring, and storing electrical energy derived from light energy."@en .

cco:ont00001139 rdf:type owl:Class ;
  rdfs:subClassOf :Vehicle ;
  rdfs:label "Spacecraft"@en ;
  rdfs:comment "Spacecraft is a Vehicle that is designed to convey passengers, cargo, or equipment from one location to another by Spaceflight."@en .

cco:ont00001024 rdf:type owl:Class ;
  rdfs:subClassOf :InternalCombustionEngine ;
  rdfs:label "Spark Ignition Engine"@en ;
  rdfs:comment "Spark Ignition Engine is an Internal Combustion Engine that is designed to operate by generating a spark to ignite a portion of Fuel and Oxidizer mixture."@en .

cco:ont00000409 rdf:type owl:Class ;
  rdfs:subClassOf :IgnitionSystem ;
  rdfs:label "Spark Ignition System"@en ;
  rdfs:comment "Spark Ignition System is an Ignition System that is designed to produce a spark in order to initiate an Ignition process."@en .

cco:ont00001000 rdf:type owl:Class ;
  rdfs:subClassOf :Nozzle ;
  rdfs:label "Spray Nozzle"@en ;
  rdfs:comment "Spray Nozzle is a Nozzle that is designed to facilitate a conversion of the flow of a portion of liquid into a dynamic collection of drops dispersed in a portion of gas."@en .

cco:ont00000634 rdf:type owl:Class ;
  rdfs:subClassOf :ExternalCombustionEngine ;
  rdfs:label "Steam Engine"@en ;
  rdfs:comment "Steam Engine is an External Combustion Engine that is designed to use steam as its working fluid."@en .

cco:ont00001019 rdf:type owl:Class ;
  rdfs:subClassOf :VehicleControlSystem ,
        [ rdf:type owl:Restriction ;
      owl:onProperty :bearer_of ;
      owl:someValuesFrom cco:ont00000679
    ] ;
  rdfs:label "Steering Control System"@en ;
  rdfs:comment "Steering Control System is a Vehicle Control System that is designed to control the direction some Vehicle is traveling."@en .

cco:ont00000054 rdf:type owl:Class ;
  rdfs:subClassOf :ExternalCombusionEngine ;
  rdfs:label "Stirling Engine"@en ;
  rdfs:comment "Stirling Engine is an External Combusion Engine that is designed to compress and expand some working fluid at different temperatures, such that there is a net conversion of heat energy to mechanical work."@en .

cco:ont00001278 rdf:type owl:Class ;
  rdfs:subClassOf :FinancialInstrument ;
  rdfs:label "Stock"@en ;
  rdfs:comment "Stock is a Financial Instrument that entitles holders to an ownership interest (equity) in the specified Incorporated Organization."@en .

cco:ont00000233 rdf:type owl:Class ;
  rdfs:subClassOf :Stock ;
  rdfs:label "Stock Certificate"@en ;
  rdfs:comment "Stock Certificate is a Stock that consists of a Certificate."@en .

cco:ont00001096 rdf:type owl:Class ;
  rdfs:subClassOf :LongGun ;
  rdfs:label "Submachine Gun"@en ;
  rdfs:comment "Submachine Gun is a Long Gun that is designed to be have automatic-fire functionality, fire pistol-caliber ammunition that is magazine-fed, and which is usually smaller than other automatic firearms."@en .

cco:ont00000728 rdf:type owl:Class ;
  rdfs:subClassOf :RadioTelescope ;
  rdfs:label "Submillimeter Wavelength Radio Telescope"@en ;
  rdfs:comment "Submillimeter Wavelength Radio Telescope is a Radio Telescope that is designed to aid in the observation of spatially distant Objects by means of collecting and focusing radio waves from the submillimeter waveband (i.e. microwaves) to form an enhanced image of the Object."@en .

cco:ont00000038 rdf:type owl:Class ;
  rdfs:subClassOf :Role ;
  rdfs:label "System Role"@en ;
  rdfs:comment "System Role is a Role that inheres in an entity in virtue of its parts or elements being arranged in such a way that they together exhibit behavior or meaning that they do not exhibit individually."@en .

cco:ont00001319 rdf:type owl:Class ;
  rdfs:subClassOf :ArmoredFightingVehicle ;
  rdfs:label "Tank"@en ;
  rdfs:comment "Tank is an Armored Fighting Vehicle that is designed to carry heavy firepower, have a powerful Engine, and travel on one or more continuous tracks such that it is suitable for front-line combat and can provide operational maneuverability as well as tactical offensive and defensive capabilities."@en .

cco:ont00001247 rdf:type owl:Class ;
  rdfs:subClassOf :TelecommunicationNetworkNode ;
  rdfs:label "Telecommunication Endpoint"@en ;
  rdfs:comment "Telecommunication Endpoint is a Telecommunication Network Node that connects a Telecommunication Terminal to a Telecommunication Network."@en .

cco:ont00000954 rdf:type owl:Class ;
  rdfs:subClassOf :InfrastructureSystem ,
        [ rdf:type owl:Restriction ;
      owl:onProperty :bearer_of ;
      owl:someValuesFrom cco:ont00000480
    ] ;
  rdfs:label "Telecommunication Infrastructure"@en ;
  rdfs:comment "Telecommunication Infrastructure is an Infrastructure System that is designed to support the use of Telecommunication Instruments to communicate."@en .

cco:ont00000690 rdf:type owl:Class ;
  rdfs:subClassOf :CommunicationInstrument ;
  rdfs:label "Telecommunication Instrument"@en ;
  rdfs:comment "Telecommunication Instrument is a Communication Instrument that is designed for use by some Agent in some Act of Communication where the recipient of that communication is potentially a significant distance away from the Agent."@en .

cco:ont00000998 rdf:type owl:Class ;
  rdfs:label "Telecommunication Network"@en ;
  rdfs:comment "A Communication System that is designed to enable the transmission of information between telecommunication endpoints via interconnected network nodes and lines."@en .

cco:ont00000825 rdf:type owl:Class ;
  rdfs:subClassOf :CommunicationArtifact ;
  rdfs:label "Telecommunication Network Line"@en ;
  rdfs:comment "Telecommunication Network Line is a Communication Artifact that is designed to be the physical transmission medium that connects two or more Telecommunication Network Nodes within a Telecommunication Network to facilitate communication between the Nodes."@en .

cco:ont00000918 rdf:type owl:Class ;
  rdfs:subClassOf :CommunicationArtifact ;
  rdfs:label "Telecommunication Network Node"@en ;
  rdfs:comment "Telecommunication Network Node is a Communication Artifact that consists of a connection point, redistribution point, or endpoint that is designed to be part of a Telecommunication Network and can be either active or passive."@en .

cco:ont00000315 rdf:type owl:Class ;
  rdfs:subClassOf :TelecommunicationNetworkNode ;
  rdfs:label "Telecommunication Switching Node"@en ;
  rdfs:comment "Telecommunication Switching Node is a Telecommunication Network Node that is capable of redirecting a communication transmission to another Telecommunication Network Node."@en .

cco:ont00000907 rdf:type owl:Class ;
  rdfs:subClassOf :TelecommunicationInstrument ;
  rdfs:label "Telephone"@en ;
  rdfs:comment "Telephone is a Telecommunication Instrument that is designed to provide point-to-point communication between agents by means of audio messages."@en .

cco:ont00000059 rdf:type owl:Class ;
  rdfs:subClassOf :TelecommunicationNetworkLine ;
  rdfs:label "Telephone Line"@en ;
  rdfs:comment "Telephone Line is a Telecommunication Network Line that consists of a physical wire or other signaling medium that is designed to be part of a Telephone Network."@en .

cco:ont00000152 rdf:type owl:Class ;
  rdfs:subClassOf :TelecommunicationNetwork ;
  rdfs:label "Telephone Network"@en ;
  rdfs:comment "Telephone Network is a Telecommunication Network that is designed to allow telephone calls to be made between two or more parties connected to the network."@en .

cco:ont00000193 rdf:type owl:Class ;
  rdfs:subClassOf :TelephoneLine ;
  rdfs:label "Telephone Subscriber Line"@en ;
  rdfs:comment "Telephone Subscriber Line is a Telephone Line that connects a Communication Endpoint to another node in a Telecommunication Network to enable service to a user's Telephone."@en .

cco:ont00000547 rdf:type owl:Class ;
  rdfs:subClassOf :ImagingInstrument ;
  rdfs:label "Telescope"@en ;
  rdfs:comment "Telescope is an Imaging Instrument that is designed to aid in the observation of spatially distant Objects by means of collecting and focusing Electromagnetic Radiation to form an enhanced image of the Object."@en .

cco:ont00000706 rdf:type owl:Class ;
  rdfs:subClassOf :MaterialArtifact ,
        [ rdf:type owl:Restriction ;
      owl:onProperty :bearer_of ;
      owl:someValuesFrom cco:ont00000098
    ] ;
  rdfs:label "Terminal Board"@en ;
  rdfs:comment "Terminal Board is a Material Artifact that is designed to join electrical terminations and create an electrical circuit by means of a block which connects individual wires without a splice or physically joining the ends."@en .

cco:ont00000018 rdf:type owl:Class ;
  rdfs:subClassOf :LegalInstrument ;
  rdfs:label "Title Document"@en ;
  rdfs:comment "Title Document is a Legal Instrument that is designed as evidence of ownership."@en .

cco:ont00000581 rdf:type owl:Class ;
  rdfs:subClassOf :MaterialArtifact ;
  rdfs:label "Tool"@en ;
  rdfs:comment "Tool is a Material Artifact that is designed to assist in the performance of manual or mechanical work and not to be consumed in that process."@en .

cco:ont00000280 rdf:type owl:Class ;
  rdfs:label "Torpedo"@en ;
  rdfs:comment "Torpedo is a Precision-Guided Missile that is designed to be fired into a body of water, be self-propelled through the water, and carry an explosive payload."@en .

cco:ont00000231 rdf:type owl:Class ;
  rdfs:subClassOf :ProjectileLauncher ;
  rdfs:label "Torpedo Tube"@en ;
  rdfs:comment "Torpedo Tube is a Projectile Launcher that is designed to launch Torpedoes."@en .

cco:ont00001201 rdf:type owl:Class ;
  rdfs:label "Trail"@en ;
  rdfs:comment "A Land Transportation Artifact that is designed to enable pedestrian or non-motorized travel through natural or constructed environments, including forests, moors, or urban greenways."@en .

cco:ont00001030 rdf:type owl:Class ;
  rdfs:subClassOf :RailTransportVehicle ;
  rdfs:label "Train"@en ;
  rdfs:comment "Train is a Rail Transport Vehicle that consists of a series of connected Train Cars or Railcars."@en .

cco:ont00000928 rdf:type owl:Class ;
  rdfs:subClassOf :RailTransportVehicle ;
  rdfs:label "Train Car"@en ;
  rdfs:comment "Train Car is a Rail Transport Vehicle that consists of a single Vehicle that is not a Train but is designed to be connected to other Train Cars along with at least one Locomotive to form a Train."@en .

cco:ont00000736 rdf:type owl:Class ;
  rdfs:subClassOf :MaterialArtifact ;
  rdfs:label "Transducer"@en ;
  rdfs:comment "Transducer is a Material Artifact that is designed to convert one form of energy to another."@en .

cco:ont00000254 rdf:type owl:Class ;
  rdfs:subClassOf :MaterialArtifact ;
  rdfs:label "Transportation Artifact"@en ;
  rdfs:comment "Transportation Artifact is a Material Artifact that is fixed in place and designed to enable the movement of Vehicles and Agents from one location to another."@en .

cco:ont00000328 rdf:type owl:Class ;
  rdfs:label "Transportation Infrastructure"@en ;
  rdfs:comment "An Infrastructure System that has continuant part one or more Transportation Artifacts and bears a function that, if realized, is realized in acts of transportation of passengers and/or cargo."@en .

cco:ont00001027 rdf:type owl:Class ;
  rdfs:subClassOf :ControlSurface ;
  rdfs:label "Trim Tab"@en ;
  rdfs:comment "Trim Tab is a Control Surface that is designed to counteract hydro-, aerodynamic, or other forces in order to stabilize the Vehicle it is part of in the desired Attitude."@en .

cco:ont00001181 rdf:type owl:Class ;
  rdfs:subClassOf :InertialNavigationSystem ;
  rdfs:label "Triple Inertial Navigation System"@en ;
  rdfs:comment "Triple Inertial Navigation System is an Inertial Navigation System that is designed to use three redundant computers to continuously calculate via dead reckoning the position, orientation, and velocity of a moving object without the need for external references, in such a way that eliminates the need for a navigator."@en .

cco:ont00000488 rdf:type owl:Class ;
  rdfs:subClassOf :MaterialArtifact ,
        [ rdf:type owl:Restriction ;
      owl:onProperty :bearer_of ;
      owl:someValuesFrom cco:ont00000480
    ] ;
  rdfs:label "Tripod"@en ;
  rdfs:comment "Tripod is a Material Artifact that consists of three legs and a platform that joins them and which is designed to support the weight and maintain the stability of objects that are attached to or rested on the platform."@en .

cco:ont00000606 rdf:type owl:Class ;
  rdfs:subClassOf :GroundMotorVehicle ;
  rdfs:label "Truck"@en ;
  rdfs:comment "Truck is a Ground Motor Vehicle that is designed to be used to transport cargo."@en .

cco:ont00000704 rdf:type owl:Class ;
  rdfs:subClassOf     [ rdf:type owl:Restriction ;
      owl:onProperty :bearer_of ;
      owl:someValuesFrom cco:ont00000650
    ] ;
  rdfs:label "Tunnel"@en ;
  rdfs:comment "A Land Transportation Artifact that is designed to enable ground vehicles to travel beneath surrounding soil, rock, or a water body (including riverbeds or seabeds)."@en .

cco:ont00000788 rdf:type owl:Class ;
  rdfs:subClassOf :SteamEngine ;
  rdfs:label "Turbine Steam Engine"@en ;
  rdfs:comment "Turbine Steam Engine is a Steam Engine that is designed to extract thermal energy from pressurized steam and use it to do mechanical work on a rotating output shaft."@en .

cco:ont00000688 rdf:type owl:Class ;
  rdfs:label "Turbofan Air-Breathing Jet Engine"@en ;
  rdfs:comment "Turbofan Air-Breathing Jet Engine is an Air-Breathing Jet Engine that uses a Turbofan, which consists of a Turbine and a Fan."@en .

cco:ont00001005 rdf:type owl:Class ;
  rdfs:label "Turbojet Air-Breathing Jet Engine"@en ;
  rdfs:comment "Turbojet Air-Breathing Jet Engine is an Air-Breathing Jet Engine that uses a Turbojet, which consists of a Turbine with a Propelling Nozzle."@en .

cco:ont00000857 rdf:type owl:Class ;
  rdfs:label "Ultra High Frequency Communication Instrument"@en ;
  rdfs:comment "A Radio Communication Instrument that is designed to transmit and/or receive radio signals in the ultra high frequency (UHF) band."@en .

cco:ont00000174 rdf:type owl:Class ;
  rdfs:subClassOf :Telescope ;
  rdfs:label "Ultraviolet Telescope"@en ;
  rdfs:comment "Ultraviolet Telescope is a Telescope that is designed to aid in the observation of spatially distant Objects by means of collecting and focusing ultraviolet light to form an enhanced image of the Object."@en .

cco:ont00001029 rdf:type owl:Class ;
  rdfs:subClassOf :PortionofAmmunition ;
  rdfs:label "Unguided Rocket"@en ;
  rdfs:comment "Unguided Rocket is a Portion of Ammunition that is designed to be a self-propelled, but unguided, projectile that delivers some payload (explosive or other) over relatively long distances through the use of a Rocket Engine."@en .

cco:ont00000598 rdf:type owl:Class ;
  rdfs:subClassOf :FluidControlArtifact ;
  rdfs:label "Valve"@en ;
  rdfs:comment "Valve is a Fluid Control Artifact that is designed to regulate, direct, or control the flow of fluid by opening, closing, or partially obstructing the fluid from moving along a passageway."@en .

cco:ont00000713 rdf:type owl:Class ;
  rdfs:subClassOf :MaterialArtifact ;
  rdfs:label "Vehicle"@en ;
  rdfs:comment "Vehicle is a Material Artifact that is designed to facilitate the movement of material entities from one location to another by conveying them there."@en .

cco:ont00000103 rdf:type owl:Class ;
  rdfs:subClassOf :MaterialArtifact ;
  rdfs:label "Vehicle Compartment"@en ;
  rdfs:comment "Vehicle Compartment is a Material Artifact that is designed to partition a Vehicle into subdivisions for various purposes."@en .

cco:ont00000723 rdf:type owl:Class ;
  rdfs:subClassOf :ControlSystem ;
  rdfs:label "Vehicle Control System"@en ;
  rdfs:comment "Vehicle Control System is a Control System that is designed to enable some Agent to control some Vehicle."@en .

cco:ont00001134 rdf:type owl:Class ;
  rdfs:subClassOf :MaterialArtifact ;
  rdfs:label "Vehicle Frame"@en ;
  rdfs:comment "Vehicle Frame is a Material Artifact that is designed to be the main supporting structure of some Vehicle."@en .

cco:ont00000904 rdf:type owl:Class ;
  rdfs:label "Vehicle Track"@en ;
  rdfs:comment "Vehicle Track is an Object Track for a Vehicle during some motion."@en .

cco:ont00000122 rdf:type owl:Class ;
  rdfs:subClassOf :ObjectTrackPoint ;
  rdfs:label "Vehicle Track Point"@en ;
  rdfs:comment "Vehicle Track Point is an Object Track Point that is where a Vehicle is or was located during some motion."@en .

cco:ont00000301 rdf:type owl:Class ;
  rdfs:subClassOf :PowerTransmissionArtifact ;
  rdfs:label "Vehicle Transmission"@en ;
  rdfs:comment "Vehicle Transmission is a Power Transmission Artifact that is designed to vary the output speed and torque in a rotating power transfer system."@en .

cco:ont00000050 rdf:type owl:Class ;
  rdfs:label "Very High Frequency Communication Instrument"@en ;
  rdfs:comment "A Radio Communication Instrument that is designed to transmit and/or receive radio signals in the very high frequency (VHF) band."@en .

cco:ont00000774 rdf:type owl:Class ;
  rdfs:subClassOf :Camera ;
  rdfs:label "Video Camera"@en ;
  rdfs:comment "Video Camera is a Camera that is designed to form and digitally or physically record a continuous stream of subsequent images of an entity or scene such that the images can be played back in succession as a video."@en .

cco:ont00000709 rdf:type owl:Class ;
  rdfs:subClassOf :ArtificialEye ;
  rdfs:label "Visual Prosthesis"@en ;
  rdfs:comment "Visual Prosthesis is an Artificial Eye that is designed to replace a missing eye, which performs the function of an eye."@en .

cco:ont00000549 rdf:type owl:Class ;
  rdfs:subClassOf :TransportationArtifact ;
  rdfs:label "Water Transportation Artifact"@en ;
  rdfs:comment "Water Transportation Artifact is a Transportation Artifact that facilitates the movement of Agents and Vehicles via water."@en .

cco:ont00000440 rdf:type owl:Class ;
  rdfs:subClassOf :Vehicle ;
  rdfs:label "Watercraft"@en ;
  rdfs:comment "Watercraft is a Vehicle that is designed to convey passengers, cargo, or equipment from one location to another by water travel."@en .

cco:ont00000445 rdf:type owl:Class ;
  rdfs:subClassOf :MaterialArtifact ;
  rdfs:label "Weapon"@en ;
  rdfs:comment "Weapon is a Material Artifact that is designed to destroy or inflict damage to structures or systems, or to kill or wound living things by creating specific lethal or nonlethal effects."@en .

cco:ont00000499 rdf:type owl:Class ;
  rdfs:subClassOf :RadioAntenna ;
  rdfs:label "Wire Antenna"@en ;
  rdfs:comment "Wire Antenna is a Radio Antenna that consists primarily of a length of wire."@en .

cco:ont00000701 rdf:type owl:Class ;
  rdfs:subClassOf :RadioReceiver ;
  rdfs:label "Wire Receiver"@en ;
  rdfs:comment "Wire Receiver is a Radio Receiver that uses a Wire Antenna to intercept radio signals."@en .

cco:ont00000363 rdf:type owl:Class ;
  rdfs:subClassOf :TelecommunicationNetwork ;
  rdfs:label "Wireless Telecommunication Network"@en ;
  rdfs:comment "Wireless Telecommunication Network is a Telecommunication Network that uses wireless connections to connect Telecommunication Network Nodes."@en .

cco:ont00000436 rdf:type owl:Class ;
  rdfs:subClassOf :Microscope ,
        [ rdf:type owl:Restriction ;
      owl:onProperty :bearer_of ;
      owl:someValuesFrom cco:ont00001148
    ] ;
  rdfs:label "X-ray Microscope"@en ;
  rdfs:comment "X-ray Microscope is a Microscope that is designed to use Electromagnetic Radiation in the soft X-ray band to produce a significantly enlarged image of the Object."@en .

cco:ont00000945 rdf:type owl:Class ;
  rdfs:subClassOf :Telescope ;
  rdfs:label "X-ray Telescope"@en ;
  rdfs:comment "X-ray Telescope is a Telescope that is designed to aid in the observation of spatially distant Objects by means of collecting and focusing X-rays to form an enhanced image of the Object."@en .

# Functions

cco:ont00000671 rdf:type owl:Class ;
  rdfs:label "Anti-Bacterial Artifact Function"@en ;
  rdfs:comment "Anti-Bacterial Artifact Function is an Anti-Microbial Artifact Function that is realized in a process which causes harm to, or the death of, some bacterium."@en .

cco:ont00000415 rdf:type owl:Class ;
  rdfs:subClassOf :PesticideArtifactFunction ;
  rdfs:label "Anti-Microbial Artifact Function"@en ;
  rdfs:comment "Anti-Microbial Artifact Function is a Pesticide Artifact Function that is realized in a process which causes illness in, or the death of, a microorganism."@en .

cco:ont00000323 rdf:type owl:Class ;
  rdfs:subClassOf :Function ;
  rdfs:label "Artifact Function"@en ;
  rdfs:comment "Artifact Function is a Function that inheres in some Artifact in virtue of that Artifact being designed to be used in processes that require that Function to be realized."@en .

cco:ont00000118 rdf:type owl:Class ;
  rdfs:subClassOf :DirectiveInformationContentEntity ;
  rdfs:label "Artifact Function Specification"@en ;
  rdfs:comment "Artifact Function Specification is a Directive Information Content Entity that prescribes some Artifact Function and which is part of some Artifact Model."@en .

cco:ont00000679 rdf:type owl:Class ;
  rdfs:subClassOf :ArtifactFunction ,
        [ rdf:type owl:Restriction ;
      owl:onProperty BFO:BFO_0000054 ;
      owl:someValuesFrom [ owl:intersectionOf ( BFO:BFO_0000015
                                                 [ rdf:type owl:Restriction ;
                                                   owl:onProperty BFO:BFO_0000057 ;
                                                   owl:someValuesFrom cco:ont00000877
                                                 ]
                                               ) ;
                           rdf:type owl:Class
                         ]
    ] ,
        [ rdf:type owl:Restriction ;
      owl:onProperty BFO:BFO_0000054 ;
      owl:someValuesFrom [ owl:intersectionOf ( BFO:BFO_0000015
                                                 [ rdf:type owl:Restriction ;
                                                   owl:onProperty BFO:BFO_0000057 ;
                                                   owl:someValuesFrom cco:ont00001249
                                                 ]
                                               ) ;
                           rdf:type owl:Class
                         ]
    ] ,
        [ rdf:type owl:Restriction ;
      owl:onProperty BFO:BFO_0000054 ;
      owl:someValuesFrom [ owl:intersectionOf ( BFO:BFO_0000015
                                                 [ rdf:type owl:Restriction ;
                                                   owl:onProperty BFO:BFO_0000057 ;
                                                   owl:someValuesFrom cco:ont00000453
                                                 ]
                                               ) ;
                           rdf:type owl:Class
                         ]
    ] ,
        [ rdf:type owl:Restriction ;
      owl:onProperty BFO:BFO_0000054 ;
      owl:someValuesFrom [ owl:intersectionOf ( BFO:BFO_0000015
                                                 [ rdf:type owl:Restriction ;
                                                   owl:onProperty BFO:BFO_0000057 ;
                                                   owl:someValuesFrom cco:ont00000252
                                                 ]
                                               ) ;
                           rdf:type owl:Class
                         ]
    ] ,
        [ rdf:type owl:Restriction ;
      owl:onProperty BFO:BFO_0000054 ;
      owl:someValuesFrom [ owl:intersectionOf ( BFO:BFO_0000015
                                                 [ rdf:type owl:Restriction ;
                                                   owl:onProperty BFO:BFO_0000057 ;
                                                   owl:someValuesFrom cco:ont00000012
                                                 ]
                                               ) ;
                           rdf:type owl:Class
                         ]
    ] ,
        [ rdf:type owl:Restriction ;
      owl:onProperty BFO:BFO_0000054 ;
      owl:someValuesFrom [ owl:intersectionOf ( BFO:BFO_0000015
                                                 [ rdf:type owl:Restriction ;
                                                   owl:onProperty BFO:BFO_0000057 ;
                                                   owl:someValuesFrom cco:ont00001019
                                                 ]
                                               ) ;
                           rdf:type owl:Class
                         ]
    ] ;
  rdfs:label "Attitude Control Artifact Function"@en ;
  rdfs:comment "Attitude Control Artifact Function is an Artifact Function that is realized by an Artifact participating in an attitude control process."@en .

cco:ont00001323 rdf:type owl:Class ;
  rdfs:subClassOf :ArtifactFunction ;
  rdfs:label "Bearing Artifact Function"@en ;
  rdfs:comment "Bearing Artifact Function is an Artifact Function that is realized in processes in which the Artifact constrains relative motion to only the desired motion, and reduces friction between moving parts."@en .

cco:ont00000267 rdf:type owl:Class ;
  rdfs:subClassOf :ChemicalReactionArtifactFunction ;
  rdfs:label "Catalyst Artifact Function"@en ;
  rdfs:comment "Catalyst Artifact Function is a Chemical Reaction Artifact Function that is realized in a process in which the rate of a chemical reaction is increased due to the participation of an additional substance, without that substance being consumed in the reaction."@en .

cco:ont00000791 rdf:type owl:Class ;
  rdfs:subClassOf :ArtifactFunction ;
  rdfs:label "Chemical Reaction Artifact Function"@en ;
  rdfs:comment "Chemical Reaction Artifact Function is an Artifact Function that is realized in a process that leads to the transformation of one set of chemical substances to another."@en .

cco:ont00000665 rdf:type owl:Class ;
  rdfs:subClassOf :ArtifactFunction ;
  rdfs:label "Cleaning Artifact Function"@en ;
  rdfs:comment "Cleaning Artifact Function is an Artifact Function that is realized in processes in which some Artifact is used to remove foreign objects from another object."@en .

cco:ont00000451 rdf:type owl:Class ;
  rdfs:subClassOf :ArtifactFunction ;
  rdfs:label "Collimation Artifact Function"@en ;
  rdfs:comment "Collimation Artifact Function is an Artifact Function that is realized by an Artifact participating in a collimation event in which the Artifact narrows a beam of particles or waves by either causing the spatial cross-section of the beam to become smaller or by causing the directions of motion of the beam's constituents to be aligned in a specifc direction of Motion."@en .

cco:ont00000727 rdf:type owl:Class ;
  rdfs:subClassOf :ArtifactFunction ,
        [ rdf:type owl:Restriction ;
      owl:onProperty BFO:BFO_0000054 ;
      owl:someValuesFrom [ owl:intersectionOf ( BFO:BFO_0000015
                                                 [ rdf:type owl:Restriction ;
                                                   owl:onProperty BFO:BFO_0000057 ;
                                                   owl:someValuesFrom cco:ont00000346
                                                 ]
                                               ) ;
                           rdf:type owl:Class
                         ]
    ] ,
        [ rdf:type owl:Restriction ;
      owl:onProperty BFO:BFO_0000054 ;
      owl:someValuesFrom [ owl:intersectionOf ( BFO:BFO_0000015
                                                 [ rdf:type owl:Restriction ;
                                                   owl:onProperty BFO:BFO_0000057 ;
                                                   owl:someValuesFrom cco:ont00000903
                                                 ]
                                               ) ;
                           rdf:type owl:Class
                         ]
    ] ;
  rdfs:label "Communication Artifact Function"@en ;
  rdfs:comment "Communication Artifact Function is an Artifact Function that is realized in a process in which meaningful signs are conveyed from one entity to another."@en .

cco:ont00000273 rdf:type owl:Class ;
  rdfs:subClassOf :ArtifactFunction ;
  rdfs:label "Communication Interference Artifact Function"@en ;
  rdfs:comment "Communication Interference Artifact Function is an Artifact Function that is realized during events in which an Artifact is used to interfere with the transmission of information for the purpose of preventing communication."@en .

cco:ont00000422 rdf:type owl:Class ;
  rdfs:subClassOf :ArtifactFunction ;
  rdfs:label "Communication Reception Artifact Function"@en ;
  rdfs:comment "Communication Reception Artifact Function is an Artifact Function that is realized during events in which an Artifact is used to receive information that has been transmitted for the purpose of communiction."@en .

cco:ont00001169 rdf:type owl:Class ;
  rdfs:subClassOf :ArtifactFunction ;
  rdfs:label "Communication Relay Artifact Function"@en ;
  rdfs:comment "Communication Relay Artifact Function is an Artifact Function that is realized during events in which an Artifact is used to first receive and then transmit information from one Artifact to another for the purpose of communiction."@en .

cco:ont00000932 rdf:type owl:Class ;
  rdfs:subClassOf :ArtifactFunction ;
  rdfs:label "Computing Artifact Function"@en ;
  rdfs:comment "Computing Artifact Function is an Artifact Function that is realized by an Artifact participating in a computation process."@en .

cco:ont00000651 rdf:type owl:Class ;
  rdfs:subClassOf :ArtifactFunction ;
  rdfs:label "Containing Artifact Function"@en ;
  rdfs:comment "Containing Artifact Function is an Artifact Function that is realized in a process in which one entity contains another."@en .

cco:ont00000034 rdf:type owl:Class ;
  rdfs:subClassOf :MotionArtifactFunction ;
  rdfs:label "Conveyance Artifact Function"@en ;
  rdfs:comment "Conveyance Artifact Function is a Motion Artifact Function that is realized in a process in which the bearer of the function conveys entities from one location to another."@en .

cco:ont00000002 rdf:type owl:Class ;
  rdfs:subClassOf :ArtifactFunction ;
  rdfs:label "Cooling Artifact Function"@en ;
  rdfs:comment "Cooling Artifact Function is an Artifact Function that is realized in a process in which the thermal energy of a system decreases."@en .

cco:ont00001310 rdf:type owl:Class ;
  rdfs:subClassOf :ArtifactFunction ;
  rdfs:label "Covering Artifact Function"@en ;
  rdfs:comment "Covering Artifact Function is an Artifact Function that is realized in a process in which an entity is covered."@en .

cco:ont00001233 rdf:type owl:Class ;
  rdfs:subClassOf :DamagingArtifactFunction ;
  rdfs:label "Crushing Artifact Function"@en ;
  rdfs:comment "Crushing Artifact Function is a Damaging Artifact Function that is realized in a process in which the structural integrity of an entity is impaired because of significant pressure."@en .

cco:ont00000961 rdf:type owl:Class ;
  rdfs:subClassOf :ElectricalArtifactFunction ;
  rdfs:label "Current Conversion Artifact Function"@en ;
  rdfs:comment "Current Conversion Artifact Function is an Electrical Artifact Function that is realized by processes in which some Artifact is used to convert some electrical current."@en .

cco:ont00000534 rdf:type owl:Class ;
  rdfs:subClassOf :DamagingArtifactFunction ;
  rdfs:label "Cutting Artifact Function"@en ;
  rdfs:comment "Cutting Artifact Function is a Damaging Artifact Function that is realized in a process in which the structural integrity of an entity is impaired by being opened or divided."@en .

cco:ont00001153 rdf:type owl:Class ;
  rdfs:subClassOf :ArtifactFunction ;
  rdfs:label "Damaging Artifact Function"@en ;
  rdfs:comment "Damaging Artifact Function is an Artifact Function that is realized in a process in which the structural integrity of an entity is impaired."@en .

cco:ont00000629 rdf:type owl:Class ;
  rdfs:subClassOf :ArtifactFunction ;
  rdfs:label "Deception Artifact Function"@en ;
  rdfs:comment "Deception Artifact Function is an Artifact Function that is realized in processes which misinform or mislead some other entity."@en .

cco:ont00000538 rdf:type owl:Class ;
  rdfs:subClassOf :HerbicideArtifactFunction ;
  rdfs:label "Defoliant Artifact Function"@en ;
  rdfs:comment "Defoliant Artifact Function is a Herbicide Artifact Function that is realized in a process that causes a plant to lose its leaves."@en .

cco:ont00000171 rdf:type owl:Class ;
  rdfs:subClassOf :SurfactantArtifactFunction ;
  rdfs:label "Detergent Artifact Function"@en ;
  rdfs:comment "Detergent Artifact Function is a Surfactant Artifact Function that is realized in a process that cleans substances in dilute solutions."@en .

cco:ont00000491 rdf:type owl:Class ;
  rdfs:subClassOf :ArtifactFunction ;
  rdfs:label "Detonating Artifact Function"@en ;
  rdfs:comment "Detonating Artifact Function is an Artifact Function that is realized in processes of combustion involving a supersonic exothermic front accelerating through a medium that eventually drives a shock front propagating directly in front of it."@en .

cco:ont00000403 rdf:type owl:Class ;
  rdfs:subClassOf :ArtifactFunction ;
  rdfs:label "Diffraction Artifact Function"@en ;
  rdfs:comment "Diffraction Artifact Function is an Artifact Function that is realized by an Artifact participating in a diffraction event in which the Artifact forces a wave to bend around the corners of an obstacle or aperture into the region of geometrical shadow of the obstacle."@en .

cco:ont00000657 rdf:type owl:Class ;
  rdfs:subClassOf :MeasurementArtifactFunction ;
  rdfs:label "Distance Measurement Artifact Function"@en ;
  rdfs:comment "Distance Measurement Artifact Function is a Measurement Artifact Function that is realized during events in which an Artifact is used to measure the spatial Distance to a specified object or class of objects."@en .

cco:ont00001329 rdf:type owl:Class ;
  rdfs:subClassOf :ServiceArtifactFunction ;
  rdfs:label "Education Artifact Function"@en ;
  rdfs:comment "Education Artifact Function is a Service Artifact Function that is realized in processes of transmiting accumulated knowledge skills and values from one generation to another."@en .

cco:ont00000098 rdf:type owl:Class ;
  rdfs:subClassOf :ArtifactFunction ,
        [ rdf:type owl:Restriction ;
      owl:onProperty BFO:BFO_0000054 ;
      owl:someValuesFrom [ owl:intersectionOf ( BFO:BFO_0000015
                                                 [ rdf:type owl:Restriction ;
                                                   owl:onProperty BFO:BFO_0000057 ;
                                                   owl:someValuesFrom cco:ont00000952
                                                 ]
                                               ) ;
                           rdf:type owl:Class
                         ]
    ] ,
        [ rdf:type owl:Restriction ;
      owl:onProperty BFO:BFO_0000054 ;
      owl:someValuesFrom [ owl:intersectionOf ( BFO:BFO_0000015
                                                 [ rdf:type owl:Restriction ;
                                                   owl:onProperty BFO:BFO_0000057 ;
                                                   owl:someValuesFrom cco:ont00000130
                                                 ]
                                               ) ;
                           rdf:type owl:Class
                         ]
    ] ,
        [ rdf:type owl:Restriction ;
      owl:onProperty BFO:BFO_0000054 ;
      owl:someValuesFrom [ owl:intersectionOf ( BFO:BFO_0000015
                                                 [ rdf:type owl:Restriction ;
                                                   owl:onProperty BFO:BFO_0000057 ;
                                                   owl:someValuesFrom cco:ont00000706
                                                 ]
                                               ) ;
                           rdf:type owl:Class
                         ]
    ] ;
  rdfs:label "Electrical Artifact Function"@en ;
  rdfs:comment "Electrical Artifact Function is an Artifact Function that is realized during events in which an Artifact is used to perform a process involving electrical power."@en .

cco:ont00000795 rdf:type owl:Class ;
  rdfs:subClassOf :ElectricalArtifactFunction ;
  rdfs:label "Electrical Conduction Artifact Function"@en ;
  rdfs:comment "Electrical Conduction Artifact Function is an Electrical Artifact Function that is realized by an Artifact being used to conduct an electric current."@en .

cco:ont00000162 rdf:type owl:Class ;
  rdfs:subClassOf :ElectricalConductionArtifactFunction ;
  rdfs:label "Electrical Connector Artifact Function"@en ;
  rdfs:comment "Electrical Connector Artifact Function is an Electrical Conduction Artifact Function that is realized by processes in which some Artifact is used to join electrical terminations to create an electrical circuit."@en .

cco:ont00000194 rdf:type owl:Class ;
  rdfs:subClassOf :ElectricalConductionArtifactFunction ;
  rdfs:label "Electrical Contact Artifact Function"@en ;
  rdfs:comment "Electrical Contact Artifact Function is an Electrical Conduction Artifact Function that is realized by processes in which some Artifact is used as an endpoint of an electrical circuit from which an electrical current is passed via physical contact with the endpoint."@en .

cco:ont00000994 rdf:type owl:Class ;
  rdfs:subClassOf :ElectricalArtifactFunction ,
        [ rdf:type owl:Restriction ;
      owl:onProperty BFO:BFO_0000054 ;
      owl:someValuesFrom [ owl:intersectionOf ( BFO:BFO_0000015
                                                 [ rdf:type owl:Restriction ;
                                                   owl:onProperty BFO:BFO_0000057 ;
                                                   owl:someValuesFrom cco:ont00000302
                                                 ]
                                               ) ;
                           rdf:type owl:Class
                         ]
    ] ,
        [ rdf:type owl:Restriction ;
      owl:onProperty BFO:BFO_0000054 ;
      owl:someValuesFrom [ owl:intersectionOf ( BFO:BFO_0000015
                                                 [ rdf:type owl:Restriction ;
                                                   owl:onProperty BFO:BFO_0000057 ;
                                                   owl:someValuesFrom cco:ont00000840
                                                 ]
                                               ) ;
                           rdf:type owl:Class
                         ]
    ] ,
        [ rdf:type owl:Restriction ;
      owl:onProperty BFO:BFO_0000054 ;
      owl:someValuesFrom [ owl:intersectionOf ( BFO:BFO_0000015
                                                 [ rdf:type owl:Restriction ;
                                                   owl:onProperty BFO:BFO_0000057 ;
                                                   owl:someValuesFrom cco:ont00000790
                                                 ]
                                               ) ;
                           rdf:type owl:Class
                         ]
    ] ,
        [ rdf:type owl:Restriction ;
      owl:onProperty BFO:BFO_0000054 ;
      owl:someValuesFrom [ owl:intersectionOf ( BFO:BFO_0000015
                                                 [ rdf:type owl:Restriction ;
                                                   owl:onProperty BFO:BFO_0000057 ;
                                                   owl:someValuesFrom cco:ont00000716
                                                 ]
                                               ) ;
                           rdf:type owl:Class
                         ]
    ] ,
        [ rdf:type owl:Restriction ;
      owl:onProperty BFO:BFO_0000054 ;
      owl:someValuesFrom [ owl:intersectionOf ( BFO:BFO_0000015
                                                 [ rdf:type owl:Restriction ;
                                                   owl:onProperty BFO:BFO_0000057 ;
                                                   owl:someValuesFrom cco:ont00000909
                                                 ]
                                               ) ;
                           rdf:type owl:Class
                         ]
    ] ,
        [ rdf:type owl:Restriction ;
      owl:onProperty BFO:BFO_0000054 ;
      owl:someValuesFrom [ owl:intersectionOf ( BFO:BFO_0000015
                                                 [ rdf:type owl:Restriction ;
                                                   owl:onProperty BFO:BFO_0000057 ;
                                                   owl:someValuesFrom cco:ont00000053
                                                 ]
                                               ) ;
                           rdf:type owl:Class
                         ]
    ] ,
        [ rdf:type owl:Restriction ;
      owl:onProperty BFO:BFO_0000054 ;
      owl:someValuesFrom [ owl:intersectionOf ( BFO:BFO_0000015
                                                 [ rdf:type owl:Restriction ;
                                                   owl:onProperty BFO:BFO_0000057 ;
                                                   owl:someValuesFrom cco:ont00000288
                                                 ]
                                               ) ;
                           rdf:type owl:Class
                         ]
    ] ,
        [ rdf:type owl:Restriction ;
      owl:onProperty BFO:BFO_0000054 ;
      owl:someValuesFrom [ owl:intersectionOf ( BFO:BFO_0000015
                                                 [ rdf:type owl:Restriction ;
                                                   owl:onProperty BFO:BFO_0000057 ;
                                                   owl:someValuesFrom cco:ont00001192
                                                 ]
                                               ) ;
                           rdf:type owl:Class
                         ]
    ] ;
  rdfs:label "Electrical Power Production Artifact Function"@en ;
  rdfs:comment "Electrical Power Production Artifact Function is an Electrical Artifact Function that is realized during events in which an Artifact is used to generate electrical power."@en .

cco:ont00001092 rdf:type owl:Class ;
  rdfs:subClassOf :ElectricalArtifactFunction ;
  rdfs:label "Electrical Power Storage Artifact Function"@en ;
  rdfs:comment "Electrical Power Storage Artifact Function is an Electrical Artifact Function that is realized during events in which an Artifact is used to store electrical power to be released at a later time."@en .

cco:ont00000407 rdf:type owl:Class ;
  rdfs:subClassOf :ElectricalArtifactFunction ;
  rdfs:label "Electrical Resistance Artifact Function"@en ;
  rdfs:comment "Electrical Resistance Artifact Function is an Electrical Artifact Function that is realized in processes in which an Artifact opposes the flow of an electric current."@en .

cco:ont00001148 rdf:type owl:Class ;
  rdfs:subClassOf :CommunicationArtifactFunction ,
        [ rdf:type owl:Restriction ;
      owl:onProperty BFO:BFO_0000054 ;
      owl:someValuesFrom [ owl:intersectionOf ( BFO:BFO_0000015
                                                 [ rdf:type owl:Restriction ;
                                                   owl:onProperty BFO:BFO_0000057 ;
                                                   owl:someValuesFrom cco:ont00000436
                                                 ]
                                               ) ;
                           rdf:type owl:Class
                         ]
    ] ;
  rdfs:label "Electromagnetic Communication Artifact Function"@en ;
  rdfs:comment "Electromagnetic Communication Artifact Function is a Communication Artifact Function that is realized in a process that conveys meaningful signs by means of electromagnetic radiation."@en .

cco:ont00001371 rdf:type owl:Class ;
  rdfs:subClassOf :ArtifactFunction ;
  rdfs:label "Electromagnetic Induction Artifact Function"@en ;
  rdfs:comment "Electromagnetic Induction Artifact Function is an Artifact Function that is realized by processes in which some Artifact that is used to produce electromotive force across an electrical conductor due to its dynamic interaction with a magnetic field."@en .

cco:ont00001174 rdf:type owl:Class ;
  rdfs:subClassOf :ArtifactFunction ;
  rdfs:label "Electromagnetic Shielding Artifact Function"@en ;
  rdfs:comment "Electromagnetic Shielding Artifact Function is an Artifact Function that is realized in a process in which an electromagnetic field is blocked by barriers made of conductive or magnetic materials."@en .

cco:ont00000317 rdf:type owl:Class ;
  rdfs:subClassOf :SignalProcessingArtifactFunction ,
        [ rdf:type owl:Restriction ;
      owl:onProperty BFO:BFO_0000054 ;
      owl:someValuesFrom [ owl:intersectionOf ( BFO:BFO_0000015
                                                 [ rdf:type owl:Restriction ;
                                                   owl:onProperty BFO:BFO_0000057 ;
                                                   owl:someValuesFrom cco:ont00000285
                                                 ]
                                               ) ;
                           rdf:type owl:Class
                         ]
    ] ;
  rdfs:label "Electronic Signal Processing Artifact Function"@en ;
  rdfs:comment "Electronic Signal Processing Artifact Function is a Signal Processing Artifact Function that inheres in Artifacts that are designed to process or transfer information contained in electronic signals."@en .

cco:ont00001281 rdf:type owl:Class ;
  rdfs:subClassOf :ChemicalReactionArtifactFunction ;
  rdfs:label "Emulsifier Artifact Function"@en ;
  rdfs:comment "Emulsifier Artifact Function is a Chemical Reaction Artifact Function that is realized in a process in which two or more liquids that are normally immiscible are mixed."@en .

cco:ont00000437 rdf:type owl:Class ;
  rdfs:subClassOf :ArtifactFunction ;
  rdfs:label "Enhancing Artifact Function"@en ;
  rdfs:comment "Enhancing Artifact Function is an Artifact Function that is realized in processes of intensifying, increainsg, or further improving the quality, value, or extent of some entity."@en .

cco:ont00000841 rdf:type owl:Class ;
  rdfs:subClassOf :DamagingArtifactFunction ;
  rdfs:label "Explosive Artifact Function"@en ;
  rdfs:comment "Explosive Artifact Function is a Damaging Artifact Function that is realized in a process in which the structural integrity of an entity is impaired because of the rapid increase in volume and release of energy in an extreme manner."@en .

cco:ont00001372 rdf:type owl:Class ;
  rdfs:subClassOf :EnhancingArtifactFunction ;
  rdfs:label "Fertilizer Artifact Function"@en ;
  rdfs:comment "Fertilizer Artifact Function is an Enhancing Artifact Function that is realized in processes of supplying soilds or plant tissues with one or more plant nutrients essential to growth."@en .

cco:ont00001999 rdf:type owl:Class ;
  rdfs:subClassOf :ArtifactFunction ;
  rdfs:label "Filter Function"@en ;
  rdfs:comment "Filter Function is an Artifact Function that is realized in a process where entities of a specific type or which have specified properties enter it or pass through it."@en .

cco:ont00000311 rdf:type owl:Class ;
  rdfs:subClassOf :FilterFunction ;
  rdfs:label "Filtration Artifact Function"@en ;
  rdfs:comment "Filtration Artifact Function is a Filter Function that is realized in a process in which some solid entity is prevented from moving along with some quantity of liquid."@en .

cco:ont00000938 rdf:type owl:Class ;
  rdfs:subClassOf :ServiceArtifactFunction ;
  rdfs:label "Financial Artifact Function"@en ;
  rdfs:comment "Financial Artifact Function is a Service Artifact Function that is realized in processes of managing money."@en .

cco:ont00001070 rdf:type owl:Class ;
  rdfs:subClassOf :ArtifactFunction ;
  rdfs:label "Fluid Control Artifact Function"@en ;
  rdfs:comment "Fluid Control Artifact Function is an Artifact Function that is realized in processes in which some Artifact is used to control the direction or flow of some fluid."@en .

cco:ont00000244 rdf:type owl:Class ;
  rdfs:subClassOf :DamagingArtifactFunction ;
  rdfs:label "Fragmentation Artifact Function"@en ;
  rdfs:comment "Fragmentation Artifact Function is a Damaging Artifact Function that is realized in a process in which the structural integrity of an entity is impaired because of a detonation which causes fragmentation."@en .

cco:ont00000183 rdf:type owl:Class ;
  rdfs:subClassOf :ArtifactFunction ;
  rdfs:label "Fragrance Artifact Function"@en ;
  rdfs:comment "Fragrance Artifact Function is an Artifact Function that is realized in processes of emitting a pleasant or sweet odor."@en .

cco:ont00000062 rdf:type owl:Class ;
  rdfs:subClassOf :MeasurementArtifactFunction ;
  rdfs:label "Frequency Measurement Artifact Function"@en ;
  rdfs:comment "Frequency Measurement Artifact Function is a Measurement Artifact Function that is realized during events in which an Artifact is used to measure the Frequency of a specified object or class of objects."@en .

cco:ont00000206 rdf:type owl:Class ;
  rdfs:subClassOf :ArtifactFunction ;
  rdfs:label "Friction Reduction Artifact Function"@en ;
  rdfs:comment "Friction Reduction Artifact Function is an Artifact Function that is realized in processes of reducing the force resisting the relative motion of surfaces in contact."@en .

cco:ont00001253 rdf:type owl:Class ;
  rdfs:subClassOf :ArtifactFunction ;
  rdfs:label "Fuel Artifact Function"@en ;
  rdfs:comment "Fuel Artifact Function is an Artifact Function that is realized in processes in which a Portion of Fuel is reacted with other substances in order to release chemical or nuclear energy to be used for heat or for work."@en .

cco:ont00001155 rdf:type owl:Class ;
  rdfs:subClassOf :ImagingArtifactFunction ,
        [ rdf:type owl:Restriction ;
      owl:onProperty BFO:BFO_0000054 ;
      owl:someValuesFrom [ owl:intersectionOf ( BFO:BFO_0000015
                                                 [ rdf:type owl:Restriction ;
                                                   owl:onProperty BFO:BFO_0000057 ;
                                                   owl:someValuesFrom cco:ont00000342
                                                 ]
                                               ) ;
                           rdf:type owl:Class
                         ]
    ] ,
        [ rdf:type owl:Restriction ;
      owl:onProperty BFO:BFO_0000054 ;
      owl:someValuesFrom [ owl:intersectionOf ( BFO:BFO_0000015
                                                 [ rdf:type owl:Restriction ;
                                                   owl:onProperty BFO:BFO_0000057 ;
                                                   owl:someValuesFrom cco:ont00001370
                                                 ]
                                               ) ;
                           rdf:type owl:Class
                         ]
    ] ,
        [ rdf:type owl:Restriction ;
      owl:onProperty BFO:BFO_0000054 ;
      owl:someValuesFrom [ owl:intersectionOf ( BFO:BFO_0000015
                                                 [ rdf:type owl:Restriction ;
                                                   owl:onProperty BFO:BFO_0000057 ;
                                                   owl:someValuesFrom cco:ont00000238
                                                 ]
                                               ) ;
                           rdf:type owl:Class
                         ]
    ] ,
        [ rdf:type owl:Restriction ;
      owl:onProperty BFO:BFO_0000054 ;
      owl:someValuesFrom [ owl:intersectionOf ( BFO:BFO_0000015
                                                 [ rdf:type owl:Restriction ;
                                                   owl:onProperty BFO:BFO_0000057 ;
                                                   owl:someValuesFrom cco:ont00000116
                                                 ]
                                               ) ;
                           rdf:type owl:Class
                         ]
    ] ;
  rdfs:label "Full Motion Video Imaging Artifact Function"@en ;
  rdfs:comment "Full Motion Video Imaging Artifact Function is an Imaging Artifact Function that inheres in Artifacts that are designed to produce video of entities that is of high enough quality to make the represented motion appear continuous to human viewers."@en .

cco:ont00000762 rdf:type owl:Class ;
  rdfs:label "Fungicide Artifact Function"@en ;
  rdfs:comment "Fungicide Artifact Function is an Anti-Microbial Artifact Function that is realized in a process which causes harm to, or the death of, some fungus or fungal spore."@en .

cco:ont00000661 rdf:type owl:Class ;
  rdfs:subClassOf :ServiceArtifactFunction ;
  rdfs:label "Government Artifact Function"@en ;
  rdfs:comment "Government Artifact Function is a Service Artifact Function that is realized in processes in which public policy is administered and the actions of its members are directed."@en .

cco:ont00000650 rdf:type owl:Class ;
  rdfs:subClassOf :MovingTargetIndicationArtifactFunction ,
        [ rdf:type owl:Restriction ;
      owl:onProperty BFO:BFO_0000054 ;
      owl:someValuesFrom [ owl:intersectionOf ( BFO:BFO_0000015
                                                 [ rdf:type owl:Restriction ;
                                                   owl:onProperty BFO:BFO_0000057 ;
                                                   owl:someValuesFrom cco:ont00000646
                                                 ]
                                               ) ;
                           rdf:type owl:Class
                         ]
    ] ,
        [ rdf:type owl:Restriction ;
      owl:onProperty BFO:BFO_0000054 ;
      owl:someValuesFrom [ owl:intersectionOf ( BFO:BFO_0000015
                                                 [ rdf:type owl:Restriction ;
                                                   owl:onProperty BFO:BFO_0000057 ;
                                                   owl:someValuesFrom cco:ont00000956
                                                 ]
                                               ) ;
                           rdf:type owl:Class
                         ]
    ] ,
        [ rdf:type owl:Restriction ;
      owl:onProperty BFO:BFO_0000054 ;
      owl:someValuesFrom [ owl:intersectionOf ( BFO:BFO_0000015
                                                 [ rdf:type owl:Restriction ;
                                                   owl:onProperty BFO:BFO_0000057 ;
                                                   owl:someValuesFrom cco:ont00001178
                                                 ]
                                               ) ;
                           rdf:type owl:Class
                         ]
    ] ,
        [ rdf:type owl:Restriction ;
      owl:onProperty BFO:BFO_0000054 ;
      owl:someValuesFrom [ owl:intersectionOf ( BFO:BFO_0000015
                                                 [ rdf:type owl:Restriction ;
                                                   owl:onProperty BFO:BFO_0000057 ;
                                                   owl:someValuesFrom cco:ont00000247
                                                 ]
                                               ) ;
                           rdf:type owl:Class
                         ]
    ] ,
        [ rdf:type owl:Restriction ;
      owl:onProperty BFO:BFO_0000054 ;
      owl:someValuesFrom [ owl:intersectionOf ( BFO:BFO_0000015
                                                 [ rdf:type owl:Restriction ;
                                                   owl:onProperty BFO:BFO_0000057 ;
                                                   owl:someValuesFrom cco:ont00001086
                                                 ]
                                               ) ;
                           rdf:type owl:Class
                         ]
    ] ,
        [ rdf:type owl:Restriction ;
      owl:onProperty BFO:BFO_0000054 ;
      owl:someValuesFrom [ owl:intersectionOf ( BFO:BFO_0000015
                                                 [ rdf:type owl:Restriction ;
                                                   owl:onProperty BFO:BFO_0000057 ;
                                                   owl:someValuesFrom cco:ont00000704
                                                 ]
                                               ) ;
                           rdf:type owl:Class
                         ]
    ] ;
  rdfs:label "Ground Moving Target Indication Artifact Function"@en ;
  rdfs:comment "Ground Moving Target Indication Artifact Function is a Moving Target Indication Artifact Function that inheres in Artifacts that are designed to identify and track entities moving on or near the ground."@en .

cco:ont00001361 rdf:type owl:Class ;
  rdfs:subClassOf :ArtifactFunction ;
  rdfs:label "Healing Artifact Function"@en ;
  rdfs:comment "Healing Artifact Function is an Artifact Function that is realized in a process in which health is restored to an unbalanced, diseased, or damaged organism."@en .

cco:ont00000309 rdf:type owl:Class ;
  rdfs:subClassOf :ServiceArtifactFunction ;
  rdfs:label "Healthcare Artifact Function"@en ;
  rdfs:comment "Healthcare Artifact Function is a Service Artifact Function that is realized in processes of treating and preventing illness."@en .

cco:ont00001013 rdf:type owl:Class ;
  rdfs:subClassOf :ArtifactFunction ;
  rdfs:label "Heating Artifact Function"@en ;
  rdfs:comment "Heating Artifact Function is an Artifact Function that is realized in a process in which the thermal energy of a system increases."@en .

cco:ont00000831 rdf:type owl:Class ;
  rdfs:subClassOf :PesticideArtifactFunction ;
  rdfs:label "Herbicide Artifact Function"@en ;
  rdfs:comment "Herbicide Artifact Function is a Pesticide Artifact Function that is realized in a process which causes harm to, or the death to, unwanted plants."@en .

cco:ont00001378 rdf:type owl:Class ;
  rdfs:subClassOf :ServiceArtifactFunction ;
  rdfs:label "Hospitality Artifact Function"@en ;
  rdfs:comment "Hospitality Artifact Function is a Service Artifact Function that is realized in processes of accommodation food and beverage meeting and events gaming entertainment and recreation tourism services and visitor information."@en .

cco:ont00000601 rdf:type owl:Class ;
  rdfs:subClassOf :ArtifactFunction ;
  rdfs:label "Imaging Artifact Function"@en ;
  rdfs:comment "Imaging Artifact Function is an Artifact Function that inheres in Artifacts that are designed to produce visual representations of entities."@en .

cco:ont00000623 rdf:type owl:Class ;
  rdfs:subClassOf :ArtifactFunction ;
  rdfs:label "Impact Shielding Artifact Function"@en ;
  rdfs:comment "Impact Shielding Artifact Function is an Artifact Function that is realized during events in which an Artifact reduces the damage caused to the shielded object by an impact with another object."@en .

cco:ont00000937 rdf:type owl:Class ;
  rdfs:subClassOf :ArtifactFunction ;
  rdfs:label "Inhibiting Motion Artifact Function"@en ;
  rdfs:comment "Inhibiting Motion Artifact Function is an Artifact Function that is realized by processes in which some Artifact is used to inhibit the motion of some object."@en .

cco:ont00001255 rdf:type owl:Class ;
  rdfs:subClassOf :PesticideArtifactFunction ;
  rdfs:label "Insecticide Artifact Function"@en ;
  rdfs:comment "Insecticide Artifact Function is a Pesticide Artifact Function that is realized in a process that causes harm to, or the death of, an insect."@en .

cco:ont00000600 rdf:type owl:Class ;
  rdfs:subClassOf :ServiceArtifactFunction ;
  rdfs:label "Legal Artifact Function"@en ;
  rdfs:comment "Legal Artifact Function is a Service Artifact Function that is realized in processes of giving legal advice to clients drafting legal documents for clients and representing clients in legal negotiations and court proceedings such as lawsuits."@en .

cco:ont00000480 rdf:type owl:Class ;
  rdfs:subClassOf :ArtifactFunction ,
        [ rdf:type owl:Restriction ;
      owl:onProperty BFO:BFO_0000054 ;
      owl:someValuesFrom [ owl:intersectionOf ( BFO:BFO_0000015
                                                 [ rdf:type owl:Restriction ;
                                                   owl:onProperty BFO:BFO_0000057 ;
                                                   owl:someValuesFrom cco:ont00001042
                                                 ]
                                               ) ;
                           rdf:type owl:Class
                         ]
    ] ,
        [ rdf:type owl:Restriction ;
      owl:onProperty BFO:BFO_0000054 ;
      owl:someValuesFrom [ owl:intersectionOf ( BFO:BFO_0000015
                                                 [ rdf:type owl:Restriction ;
                                                   owl:onProperty BFO:BFO_0000057 ;
                                                   owl:someValuesFrom cco:ont00000954
                                                 ]
                                               ) ;
                           rdf:type owl:Class
                         ]
    ] ,
        [ rdf:type owl:Restriction ;
      owl:onProperty BFO:BFO_0000054 ;
      owl:someValuesFrom [ owl:intersectionOf ( BFO:BFO_0000015
                                                 [ rdf:type owl:Restriction ;
                                                   owl:onProperty BFO:BFO_0000057 ;
                                                   owl:someValuesFrom cco:ont00000488
                                                 ]
                                               ) ;
                           rdf:type owl:Class
                         ]
    ] ;
  rdfs:label "Life Support Artifact Function"@en ;
  rdfs:comment "Life Support Artifact Function is an Artifact Function that is realized during events in which an Artifact materially affects an organism, where this causes that organism to continue living in a situation where death would otherwise occur."@en .

cco:ont00001211 rdf:type owl:Class ;
  rdfs:subClassOf :ArtifactFunction ;
  rdfs:label "Lifting Artifact Function"@en ;
  rdfs:comment "Lifting Artifact Function is an Artifact Function that is realized by processes in which some Artifact is used to lift some object."@en .

cco:ont00001365 rdf:type owl:Class ;
  rdfs:subClassOf :SpeedArtifactFunction ;
  rdfs:label "Maximum Speed Artifact Function"@en ;
  rdfs:comment "Maximum Speed Artifact Function is a Speed Artifact Function that is realized in some process in which the Artifact bearing the Artifact Function attains the highest speed at which that Artifact is designed to operate."@en .

cco:ont00001100 rdf:type owl:Class ;
  rdfs:subClassOf :ArtifactFunction ;
  rdfs:label "Measurement Artifact Function"@en ;
  rdfs:comment "Measurement Artifact Function is an Artifact Function that is realized during events in which an Artifact is used to measure one or more features of a specified object or class of objects."@en .

cco:ont00000066 rdf:type owl:Class ;
  rdfs:subClassOf :ServiceArtifactFunction ;
  rdfs:label "Military Artifact Function"@en ;
  rdfs:comment "Military Artifact Function is a Service Artifact Function that is realized in processes related to the armed services."@en .

cco:ont00000190 rdf:type owl:Class ;
  rdfs:subClassOf :SpeedArtifactFunction ;
  rdfs:label "Minimum Speed Artifact Function"@en ;
  rdfs:comment "Minimum Speed Artifact Function is a Speed Artifact Function that is realized in some process in which the Artifact bearing the Artifact Function attains the lowest speed at which that Artifact is designed to operate."@en .

cco:ont00000448 rdf:type owl:Class ;
  rdfs:subClassOf :ArtifactFunction ;
  rdfs:label "Motion Artifact Function"@en ;
  rdfs:comment "Motion Artifact Function is an Artifact Function that is realized in a process in which an entity changes its position with respect to time."@en .

cco:ont00001368 rdf:type owl:Class ;
  rdfs:subClassOf :ObservationArtifactFunction ,
        [ rdf:type owl:Restriction ;
      owl:onProperty BFO:BFO_0000054 ;
      owl:someValuesFrom [ owl:intersectionOf ( BFO:BFO_0000015
                                                 [ rdf:type owl:Restriction ;
                                                   owl:onProperty BFO:BFO_0000057 ;
                                                   owl:someValuesFrom cco:ont00001216
                                                 ]
                                               ) ;
                           rdf:type owl:Class
                         ]
    ] ;
  rdfs:label "Motion Observation Artifact Function"@en ;
  rdfs:comment "Motion Observation Artifact Function is an Observation Artifact Function that is realized during events in which an Artifact is used to collect information about the Motion of a specified object or class of objects."@en .

cco:ont00000214 rdf:type owl:Class ;
  rdfs:subClassOf :RadarImagingArtifactFunction ;
  rdfs:label "Moving Target Indication Artifact Function"@en ;
  rdfs:comment "Moving Target Indication Artifact Function is a Radar Imaging Artifact Function that inheres in Artifacts that are designed to identify and produce visual representations of moving entities by using a radar to emit successive phase coherent pulses, which are sampled and added to the subsequent pulse to cancel out signals from non-moving entities such that only signals from moving entities remain and are displayed."@en .

cco:ont00000603 rdf:type owl:Class ;
  rdfs:subClassOf :ArtifactFunction ;
  rdfs:label "Navigation Artifact Function"@en ;
  rdfs:comment "Navigation Artifact Function is an Artifact Function that is realized during events in which an Artifact is used to determine the precise location of itself or another object and plan a route to a specified destination."@en .

cco:ont00001234 rdf:type owl:Class ;
  rdfs:subClassOf :ChemicalReactionArtifactFunction ;
  rdfs:label "Neutralization Artifact Function"@en ;
  rdfs:comment "Neutralization Artifact Function is a Chemical Reaction Artifact Function that is realized in a process in which an acid and a base react quantitatively with each other."@en .

cco:ont00001275 rdf:type owl:Class ;
  rdfs:subClassOf :SpeedArtifactFunction ;
  rdfs:label "Nominal Speed Artifact Function"@en ;
  rdfs:comment "Nominal Speed Artifact Function is a Speed Artifact Function that is realized in some process in which the Artifact bearing the Artifact Function attains a speed that does not exceed some specified tolerance of that Artifact."@en .

cco:ont00001044 rdf:type owl:Class ;
  rdfs:subClassOf :ArtifactFunction ;
  rdfs:label "Nuclear Radiation Detection Artifact Function"@en ;
  rdfs:comment "Nuclear Radiation Detection Artifact Function is an Artifact Function that is realized during events in which an Artifact is used to detect the presence of nuclear radiation particles."@en .

cco:ont00001306 rdf:type owl:Class ;
  rdfs:subClassOf :ArtifactFunction ;
  rdfs:label "Observation Artifact Function"@en ;
  rdfs:comment "Observation Artifact Function is an Artifact Function that is realized during events in which an Artifact is used to collect information about a specified object or class of objects."@en .

cco:ont00000823 rdf:type owl:Class ;
  rdfs:subClassOf :ElectromagneticCommunicationArtifactFunction ;
  rdfs:label "Optical Communication Artifact Function"@en ;
  rdfs:comment "Optical Communication Artifact Function is an Electromagnetic Communication Artifact Function that is realized in a process that conveys meaningful signs by means of visible light."@en .

cco:ont00000764 rdf:type owl:Class ;
  rdfs:subClassOf :OpticalProcessingArtifactFunction ;
  rdfs:label "Optical Focusing Artifact Function"@en ;
  rdfs:comment "Optical Focusing Artifact Function is an Optical Processing Artifact Function that is realized by an Artifact participating in a light focusing event in which the Artifact causes the light beam to converge on a target spatial point."@en .

cco:ont00000504 rdf:type owl:Class ;
  rdfs:subClassOf :ArtifactFunction ;
  rdfs:label "Optical Processing Artifact Function"@en ;
  rdfs:comment "Optical Processing Artifact Function is an Artifact Function that is realized by an Artifact participating in a visible light processing event."@en .

cco:ont00000466 rdf:type owl:Class ;
  rdfs:subClassOf :ArtifactFunction ;
  rdfs:label "Orientation Control Artifact Function"@en ;
  rdfs:comment "Orientation Control Artifact Function is an Artifact Function that is realized by processes in which some Artifact is used to control the Orientation of some object."@en .

cco:ont00001087 rdf:type owl:Class ;
  rdfs:subClassOf :ObservationArtifactFunction ;
  rdfs:label "Orientation Observation Artifact Function"@en ;
  rdfs:comment "Orientation Observation Artifact Function is an Observation Artifact Function that is realized during events in which an Artifact is used to collect information about the Orientation of a specified object or class of objects."@en .

cco:ont00000412 rdf:type owl:Class ;
  rdfs:subClassOf :ChemicalReactionArtifactFunction ;
  rdfs:label "Oxidizer Artifact Function"@en ;
  rdfs:comment "Oxidizer Artifact Function is a Chemical Reaction Artifact Function that is realized in a process in which electrons are removed from a reactant in a redox reaction."@en .

cco:ont00000828 rdf:type owl:Class ;
  rdfs:subClassOf :PoisonArtifactFunction ;
  rdfs:label "Pesticide Artifact Function"@en ;
  rdfs:comment "Pesticide Artifact Function is a Poison Artifact Function that is realized in a process which causes illness in, or the death of, a living thing that is detrimental to humans or human concerns."@en .

cco:ont00001123 rdf:type owl:Class ;
  rdfs:subClassOf :DamagingArtifactFunction ;
  rdfs:label "Poison Artifact Function"@en ;
  rdfs:comment "Poison Artifact Function is a Damaging Artifact Function that is realized in a process which causes illness in, or the death of, a living thing."@en .

cco:ont00001303 rdf:type owl:Class ;
  rdfs:subClassOf :ObservationArtifactFunction ;
  rdfs:label "Position Observation Artifact Function"@en ;
  rdfs:comment "Position Observation Artifact Function is an Observation Artifact Function that is realized during events in which an Artifact is used to collect information about the position of a specified object or class of objects."@en .

cco:ont00000019 rdf:type owl:Class ;
  rdfs:subClassOf :CurrentConversionArtifactFunction ;
  rdfs:label "Power Inverting Artifact Function"@en ;
  rdfs:comment "Power Inverting Artifact Function is a Current Conversion Artifact Function that is realized by processes in which some Artifact is used to convert direct current (DC) to alternating current (AC)."@en .

cco:ont00000993 rdf:type owl:Class ;
  rdfs:subClassOf :CurrentConversionArtifactFunction ;
  rdfs:label "Power Rectifying Artifact Function"@en ;
  rdfs:comment "Power Rectifying Artifact Function is a Current Conversion Artifact Function that is realized by processes in which some Artifact is used to convert alternating current (AC) to direct current (DC)."@en .

cco:ont00001366 rdf:type owl:Class ;
  rdfs:subClassOf :ArtifactFunction ;
  rdfs:label "Powering Artifact Function"@en ;
  rdfs:comment "Powering Artifact Function is an Artifact Function that is realized by processes in which some Artifact is used to supply power to some Artifact."@en .

cco:ont00001129 rdf:type owl:Class ;
  rdfs:subClassOf :VentilationControlArtifactFunction ;
  rdfs:label "Pressurization Control Artifact Function"@en ;
  rdfs:comment "Pressurization Control Artifact Function is a Ventilation Control Artifact Function that is realized by processes in which some Artifact is used to control the partial pressure of air in some space."@en .

cco:ont00001252 rdf:type owl:Class ;
  rdfs:subClassOf :MotionArtifactFunction ;
  rdfs:label "Propulsion Artifact Function"@en ;
  rdfs:comment "Propulsion Artifact Function is a Motion Artifact Function that is realized in a process in which the bearer of the function creates force leading to an entity's movement."@en .

cco:ont00000864 rdf:type owl:Class ;
  rdfs:subClassOf :ServiceArtifactFunction ;
  rdfs:label "Public Safety Artifact Function"@en ;
  rdfs:comment "Public Safety Artifact Function is a Service Artifact Function that is realized in processes of preventing and responding to events that could endanger the safety of the general public from significant danger, injury/harm, or damage, such as crimes or disasters (natural or man-made)."@en .

cco:ont00000289 rdf:type owl:Class ;
  rdfs:subClassOf :ImagingArtifactFunction ;
  rdfs:label "Radar Imaging Artifact Function"@en ;
  rdfs:comment "Radar Imaging Artifact Function is an Imaging Artifact Function that inheres in Artifacts that are designed to produce visual representations of entities using radio waves."@en .

cco:ont00001240 rdf:type owl:Class ;
  rdfs:subClassOf :ElectromagneticCommunicationArtifactFunction ;
  rdfs:label "Radio Communication Artifact Function"@en ;
  rdfs:comment "Radio Communication Artifact Function is an Electromagnetic Communication Artifact Function that is realized in a process that conveys meaningful signs by means of radio waves."@en .

cco:ont00000495 rdf:type owl:Class ;
  rdfs:subClassOf :CommunicationInterferenceArtifactFunction ;
  rdfs:label "Radio Communication Interference Artifact Function"@en ;
  rdfs:comment "Radio Communication Interference Artifact Function is a Communication Interference Artifact Function that is realized during events in which an Artifact is used to interfere with the transmission of information via radio waves."@en .

cco:ont00000022 rdf:type owl:Class ;
  rdfs:subClassOf :CommunicationReceptionArtifactFunction ;
  rdfs:label "Radio Communication Reception Artifact Function"@en ;
  rdfs:comment "Radio Communication Reception Artifact Function is a Communication Reception Artifact Function that is realized during events in which an Artifact receives information transmitted from another Artifact, where the transmission of information occurs using radio waves."@en .

cco:ont00000900 rdf:type owl:Class ;
  rdfs:subClassOf :CommunicationRelayArtifactFunction ;
  rdfs:label "Radio Communication Relay Artifact Function"@en ;
  rdfs:comment "Radio Communication Relay Artifact Function is a Communication Relay Artifact Function that is realized during events in which an Artifact is used to first receive and then transmit information without the use of wires from one Artifact to another for the purpose of communiction."@en .

cco:ont00000811 rdf:type owl:Class ;
  rdfs:subClassOf :ArtifactFunction ;
  rdfs:label "Radio Wave Conversion Artifact Function"@en ;
  rdfs:comment "Radio Wave Conversion Artifact Function is an Artifact Function that is realized by an Artifact being used to convert electric power into radio waves or radio waves into electric power."@en .

cco:ont00000808 rdf:type owl:Class ;
  rdfs:subClassOf :ChemicalReactionArtifactFunction ;
  rdfs:label "Reactant Artifact Function"@en ;
  rdfs:comment "Reactant Artifact Function is a Chemical Reaction Artifact Function that is realized in a process in which a substance or compound is added to a system in order to bring about a chemical reaction and is consumed in the course of the reaction."@en .

cco:ont00001085 rdf:type owl:Class ;
  rdfs:subClassOf :ArtifactFunction ;
  rdfs:label "Reflection Artifact Function"@en ;
  rdfs:comment "Reflection Artifact Function is an Artifact Function that is realized by an Artifact participating in a reflection event in which the Artifact causes a change in a wavefront at an interface between the reflecting medium and the transmission medium such that the wavefront returns into the transmission medium."@en .

cco:ont00000635 rdf:type owl:Class ;
  rdfs:subClassOf :ArtifactFunction ;
  rdfs:label "Refraction Artifact Function"@en ;
  rdfs:comment "Refraction Artifact Function is an Artifact Function that is realized by an Artifact participating in a refraction event in which the Artifact causes a change in direction of wave propagation due to a change in its transmission medium."@en .

cco:ont00000880 rdf:type owl:Class ;
  rdfs:subClassOf :ServiceArtifactFunction ;
  rdfs:label "Religious Artifact Function"@en ;
  rdfs:comment "Religious Artifact Function is a Service Artifact Function that is realized in processes related to worship and prayer."@en .

cco:ont00000481 rdf:type owl:Class ;
  rdfs:subClassOf :ServiceArtifactFunction ;
  rdfs:label "Research and Development Artifact Function"@en ;
  rdfs:comment "Research and Development Artifact Function is a Service Artifact Function that is realized in processes of producing new knowledge or of devising new applications of existing knowledge."@en .

cco:ont00000353 rdf:type owl:Class ;
  rdfs:subClassOf :ArtifactFunction ;
  rdfs:label "Research Artifact Function"@en ;
  rdfs:comment "Research Artifact Function is an Artifact Function that is realized during events in which an Artifact is used to perform research on a specified entity or class of entities."@en .

cco:ont00000321 rdf:type owl:Class ;
  rdfs:subClassOf :ServiceArtifactFunction ;
  rdfs:label "Residential Artifact Function"@en ;
  rdfs:comment "Residential Artifact Function is a Service Artifact Function that is realized in processes of residing in a dwelling or home."@en .

cco:ont00001210 rdf:type owl:Class ;
  rdfs:subClassOf :ServiceArtifactFunction ;
  rdfs:label "Retail Artifact Function"@en ;
  rdfs:comment "Retail Artifact Function is a Service Artifact Function that is realized in processes of selling goods or merchandise in small or individual lots for direct consumption by persons or organizations."@en .

cco:ont00001241 rdf:type owl:Class ;
  rdfs:subClassOf :ArtifactFunction ;
  rdfs:label "Sensor Artifact Function"@en ;
  rdfs:comment "Sensor Artifact Function is an Artifact Function that is realized in processes wherein its bearer is used to produce an output signal which reliably corresponds to changes in the artifact's environment."@en .

cco:ont00000023 rdf:type owl:Class ;
  rdfs:subClassOf :ArtifactFunction ;
  rdfs:label "Sensor Deployment Artifact Function"@en ;
  rdfs:comment "Sensor Deployment Artifact Function is an Artifact Function that inheres in Artifacts that are designed to support or convey one or more Sensors while the Sensors are realizing their own Artifact Functions."@en .

cco:ont00001273 rdf:type owl:Class ;
  rdfs:subClassOf :SensorArtifactFunction ;
  rdfs:label "Sensor Modality Function"@en ;
  rdfs:comment "Sensor Modality Function is a Sensor Artifact Function that inheres in some Sensor in virtue of the type of energy the Sensor is capable of converting into an output signal."@en .

cco:ont00001301 rdf:type owl:Class ;
  rdfs:subClassOf :ArtifactFunction ;
  rdfs:label "Service Artifact Function"@en ;
  rdfs:comment "Service Artifact Function is an Artifact Function that is realized in a process of providing intangible goods to consumers."@en .

cco:ont00000776 rdf:type owl:Class ;
  rdfs:subClassOf :ArtifactFunction ;
  rdfs:label "Signal Detection Artifact Function"@en ;
  rdfs:comment "Signal Detection Artifact Function is an Artifact Function that is realized in the process of discerning between information-bearing patterns and random patterns, or noise, that distract from the information."@en .

cco:ont00001218 rdf:type owl:Class ;
  rdfs:subClassOf :ArtifactFunction ;
  rdfs:label "Signal Processing Artifact Function"@en ;
  rdfs:comment "Signal Processing Artifact Function is an Artifact Function that is realized in the process of transferring or processing information contained in signals."@en .

cco:ont00001160 rdf:type owl:Class ;
  rdfs:subClassOf :ChemicalReactionArtifactFunction ;
  rdfs:label "Solvent Artifact Function"@en ;
  rdfs:comment "Solvent Artifact Function is a Chemical Reaction Artifact Function that is realized in the dissolving of other substances (namely, solutes) without change in the former's chemical structure."@en .

cco:ont00001353 rdf:type owl:Class ;
  rdfs:subClassOf :MotionArtifactFunction ;
  rdfs:label "Speed Artifact Function"@en ;
  rdfs:comment "Speed Artifact Function is a Motion Artifact Function that is realized in some process in which its bearer has some speed."@en .

cco:ont00000411 rdf:type owl:Class ;
  rdfs:subClassOf :MeasurementArtifactFunction ;
  rdfs:label "Speed Measurement Artifact Function"@en ;
  rdfs:comment "Speed Measurement Artifact Function is a Measurement Artifact Function that is realized during events in which an Artifact is used to measure the Speed of a specified object's or class of objects' Motion."@en .

cco:ont00001200 rdf:type owl:Class ;
  rdfs:subClassOf :ArtifactFunction ;
  rdfs:label "Structural Support Artifact Function"@en ;
  rdfs:comment "Structural Support Artifact Function is an Artifact Function that is realized by an Artifact providing physical support to another object."@en .

cco:ont00000809 rdf:type owl:Class ;
  rdfs:subClassOf :ArtifactFunction ;
  rdfs:label "Submersible Artifact Function"@en ;
  rdfs:comment "Submersible Artifact Function is an Artifact Function that is realized in processes of operating while submerged in water."@en .

cco:ont00000344 rdf:type owl:Class ;
  rdfs:subClassOf :EmulsifierArtifactFunction ;
  rdfs:label "Surfactant Artifact Function"@en ;
  rdfs:comment "Surfactant Artifact Function is an Emulsifier Artifact Function that is realized in a process that lowers the surface tension between two liquids or between a liquid and a solid."@en .

cco:ont00000689 rdf:type owl:Class ;
  rdfs:subClassOf :ArtifactFunction ;
  rdfs:label "Switch Artifact Function"@en ;
  rdfs:comment "Switch Artifact Function is an Artifact Function that is realized in a process of breaking an electric circuit by interrupting the current or diverting it from one conductor to another."@en .

cco:ont00000482 rdf:type owl:Class ;
  rdfs:subClassOf :RadarImagingArtifactFunction ;
  rdfs:label "Synthetic Aperture Radar Imaging Artifact Function"@en ;
  rdfs:comment "Synthetic Aperture Radar Imaging Artifact Function is a Radar Imaging Artifact Function that inheres in Artifacts that are designed to produce visual representations of entities using the motion of a radar antenna over a targeted region to create a synthetic aperture."@en .

cco:ont00000947 rdf:type owl:Class ;
  rdfs:subClassOf :MeasurementArtifactFunction ;
  rdfs:label "Temperature Measurement Artifact Function"@en ;
  rdfs:comment "Temperature Measurement Artifact Function is a Measurement Artifact Function that is realized during events in which an Artifact is used to measure the Temperature of a specified object or class of objects."@en .

cco:ont00001350 rdf:type owl:Class ;
  rdfs:subClassOf :ArtifactFunction ;
  rdfs:label "Thermal Control Artifact Function"@en ;
  rdfs:comment "Thermal Control Artifact Function is an Artifact Function that is realized by an Artifact increasing, decreasing, or maintaining the temperature of itself, a part of itself, or another object."@en .

cco:ont00000944 rdf:type owl:Class ;
  rdfs:subClassOf :ImagingArtifactFunction ;
  rdfs:label "Thermal Imaging Artifact Function"@en ;
  rdfs:comment "Thermal Imaging Artifact Function is an Imaging Artifact Function that is realized during events in which an Artifact is used to create a visual representation of an entity using radiation from the far infrared region of the electromagnetic spectrum that the entity emits."@en .

cco:ont00000985 rdf:type owl:Class ;
  rdfs:subClassOf :ThermalControlArtifactFunction ;
  rdfs:label "Thermal Insulation Artifact Function"@en ;
  rdfs:comment "Thermal Insulation Artifact Function is a Thermal Control Artifact Function that is realized during events in which an Artifact prevents or reduces the transfer of heat between objects that are in thermal contact or in range of radiative influence."@en .

cco:ont00000452 rdf:type owl:Class ;
  rdfs:subClassOf :ArtifactFunction ;
  rdfs:label "Timekeeping Artifact Function"@en ;
  rdfs:comment "Timekeeping Artifact Function is an Artifact Function that is realized during events in which an Artifact is used to keep track of and report the current time."@en .

cco:ont00000113 rdf:type owl:Class ;
  rdfs:subClassOf :ArtifactFunction ;
  rdfs:label "Ventilation Control Artifact Function"@en ;
  rdfs:comment "Ventilation Control Artifact Function is an Artifact Function that is realized in processes in which some Artifact is used to control the quality of air in some space."@en .

cco:ont00000678 rdf:type owl:Class ;
  rdfs:subClassOf :ArtifactFunction ;
  rdfs:label "Voltage Regulating Artifact Function"@en ;
  rdfs:comment "Voltage Regulating Artifact Function is an Artifact Function that is realized by processes in which some Artifact is used to cause a change in the voltage magnitude between the sending and receiving end of an electrical component."@en .

cco:ont00000036 rdf:type owl:Class ;
  rdfs:subClassOf :ServiceArtifactFunction ;
  rdfs:label "Waste Management Artifact Function"@en ;
  rdfs:comment "Waste Management Artifact Function is a Service Artifact Function that is realized in processes of collecting, transporting, processing, recycling, monitoring, or disposing of waste materials."@en .

cco:ont00001299 rdf:type owl:Class ;
  rdfs:subClassOf :SurfactantArtifactFunction ;
  rdfs:label "Wetting Agent Artifact Function"@en ;
  rdfs:comment "Wetting Agent Artifact Function is a Surfactant Artifact Function that is realized in a process that reduces the water repellent tendency of a substance thereby allowing it to become wet."@en .

cco:ont00000076 rdf:type owl:Class ;
  rdfs:label "Wired Communication Artifact Function"@en ;
  rdfs:comment "A Communication Artifact Function that is realized in a process that conveys meaningful signs via physical wired media, such as metallic conductors or optical fiber."@en .

cco:ont00000886 rdf:type owl:Class ;
  rdfs:subClassOf :CommunicationReceptionArtifactFunction ;
  rdfs:label "Wired Communication Reception Artifact Function"@en ;
  rdfs:comment "Wired Communication Reception Artifact Function is a Communication Reception Artifact Function that is realized during events in which an Artifact receives information transmitted from another Artifact, where the transmission of information occurs via a direct connection using an electrical conductor."@en .

cco:ont00001271 rdf:type owl:Class ;
  rdfs:subClassOf :CommunicationRelayArtifactFunction ;
  rdfs:label "Wired Communication Relay Artifact Function"@en ;
  rdfs:comment "Wired Communication Relay Artifact Function is a Communication Relay Artifact Function that is realized during events in which an Artifact is used to first receive and then transmit information by means of wires from one Artifact to another for the purpose of communiction."@en .

